Not quite finished version that pulls quantifiers over arbitrary connectives.

MirrorCharge!/src/ILPullQuant.v
@@ -19,6 +19,7 @@ Require Import ExtLib.Tactics.EqDep.
 Require Import Ext.SetoidFold.
 Require Import Relation_Definitions.
 Require Import MirrorCore.Ext.AppFull.
+Require Export ExtLib.Data.HList.
 
 Set Implicit Arguments.
 Unset Strict Implicit.
@@ -33,63 +34,18 @@ Section PullQuant.
   Context {es : embed_ops ts} {esOk : embed_opsOk gs es}.
   Context {is : inhabited ts}.
   Check logic_ops.
- 
-  Inductive variance := CoVariant | ContraVariant.
-  Inductive pull_type := PAll | PExists.
-
-  Definition TT := variance -> pull_type -> list typ * expr ilfunc.
 
   Local Instance RSym_sym : SymI.RSym (typD ts) ilfunc := RSym_ilfunc funcs gs es.
 
-  Let T:Type := tenv typ -> tenv typ -> TT.
-  Definition atomic (e : expr ilfunc) : T := fun _ _ _ _ => (nil, e).
-
-  Definition pq_var (v : var) : T := atomic (Var v).
-  Definition pq_uvar (u : uvar) : T := atomic (UVar u).
-  Definition pq_inj (s : ilfunc) : T := atomic (Inj s).
-  Definition pq_abs (x : typ) (e : expr ilfunc) (_ : T) : T :=
-    atomic (Abs x e).
-    
-  Definition pq_env := ilfunc -> variance -> pull_type -> list (option (variance * pull_type)).
-
-  Fixpoint pq_app_aux (us vs : tenv typ) (ats : list (option (variance * pull_type))) (f : list typ * expr ilfunc) (args : list (expr ilfunc * T)) : list typ * expr ilfunc :=
-  match ats, args with
-  	| Some (var, pt)::ats, (_, t)::args =>
-  	  match f, t us vs var pt with
-  	  	| (xs, f'), (ys, a) => pq_app_aux us vs ats (ys ++ xs, App (lift 0 (length ys) f') (lift (length xs) (length ys) a)) args
-  	  end
-  	| None::ats, (e, _)::args => 
-  	  match f with
-  	    | (xs, f') => pq_app_aux us vs ats (xs, App f' (lift 0 (length xs) e)) args
-  	  end
-  	| _, _ => match f with
-  			  | (xs, f') => (xs, apps f' (map fst args))
-  			  end
-  end.
-  
-  Definition pq_app (e : pq_env) (f : expr ilfunc) (_ : T) (args : list (expr ilfunc * T)) : T :=
-  	fun us vs var pt => 
-  		match f with
-  			| Inj f => pq_app_aux us vs (e f var pt) (nil, Inj f) args
-  			| _     => (nil, f)
-  		end.
  
-  Definition pq_exists (t t_logic : typ) (f : expr ilfunc) (a : T) : T :=
-    fun us vs vm pt =>
-      match pt with
-      	| PExists => let (ts, a) := a us (t :: vs) vm pt in (t::ts, a)
-      	| _       => (nil, App (Inj (ilf_exists t t_logic)) (Abs t f)) 
-      	
-      end.
-
-  Definition pqArgs (e : pq_env) : AppFullFoldArgs ilfunc TT :=
-    @Build_AppFullFoldArgs ilfunc TT pq_var pq_uvar pq_inj pq_abs (pq_app e).
-
+  Inductive variance := CoVariant | ContraVariant.
+  Inductive pull_type := PAll | PExists.
+  
   Definition get_quant (pt : pull_type) :=
   	match pt with
   	  | PAll => ilf_forall
   	  | Pexists => ilf_exists
-  	end.
+  	end.  
 
   Definition add_quant (pt : pull_type) (t : typ) (x : typ) (e : expr ilfunc) :=
     App (Inj ((get_quant pt) x t)) (Abs x e).
@@ -105,6 +61,15 @@ Section PullQuant.
     
   Require Import Morphisms.
 
+ Require Import Program.Basics.
+  
+  Definition var_entail (var : variance) (A : Type) (ILOps: ILogicOps A) :=
+  	match var with
+  	  | CoVariant => (@lentails A ILOps)
+  	  | ContraVariant => (flip lentails)
+    end.
+
+
 Section pt_quant_morphisms.
 
   Context {A : Type} `{HIL : ILogic A}.
@@ -119,6 +84,23 @@ Section pt_quant_morphisms.
     Proper (pointwise_relation T lequiv ++> lequiv) (pt_quant pt _).
   Proof.
     destruct pt; simpl; [apply @lforall_lequiv_m | apply @lexists_lequiv_m]; apply _.
+  Qed.
+
+  Global Instance var_entails_lequiv_m (vars : variance) :
+    Proper (lequiv ==> lequiv ==> iff) (var_entail vars _).
+  Proof.
+    destruct vars; simpl; apply _.
+  Qed.
+
+  Global Instance var_entails_m (vars : variance) :
+    Proper ((var_entail vars _) --> (var_entail vars _) ++> impl) (var_entail vars _).
+  Proof.
+	destruct vars; simpl; apply _.
+  Qed.
+
+  Global Instance var_entail_eq (vars : variance) : PreOrder (var_entail vars _).
+  Proof.
+	destruct vars; simpl; apply _.
   Qed.
 
 End pt_quant_morphisms.
@@ -141,15 +123,6 @@ End pt_quant_morphisms.
   
   Local Existing Instance ILFun_Ops.
   
-  Require Import Program.Basics.
-  
-  Definition var_entail (var : variance) (A : Type) (ILOps: ILogicOps A) :=
-  	match var with
-  	  | CoVariant => (@lentails A ILOps)
-  	  | ContraVariant => (flip lentails)
-    end.
-  Check @lequiv.
-  
   Inductive valid_arg (pt : pull_type) (var : variance) (t : typ) (ILOps : ILogicOps (typD ts nil t)) (A : Type) : 
     forall typs : list typ,  (A -> typD ts nil (fold_right tyArr t typs)) -> list (option (variance * pull_type)) -> Prop :=
     | ve_nil f : @valid_arg pt var t ILOps A nil f nil
@@ -158,9 +131,10 @@ End pt_quant_morphisms.
       (forall e, @valid_arg pt var t ILOps A typs (fun x => (f x) e) args) ->
       @valid_arg pt var t ILOps A (te::typs) f (None::args)
     | ve_some te typs (f : A -> typD ts nil te -> typD ts nil (fold_right tyArr t typs)) pt' var' args :
-      forall B (e : B -> typD ts nil te) (ILOps' : ILogicOps (typD ts nil te)), 
-             (var_entail var _) (((pt_quant pt) _ _ f) ((pt_quant pt') _ _ e)) ((pt_quant pt) _ _ (fun x => (pt_quant pt) _ _ (fun y => (f x) (e y)))) ->
-      @valid_arg pt var t ILOps ((A * B)%type) typs (fun x => (f (fst x)) (e (snd x))) args ->       
+      (forall B x (e : B -> typD ts nil te) (ILOps' : ILogicOps (typD ts nil te)), 
+             (var_entail var _) ((pt_quant pt) _ _ (fun y => (f x) (e y))) ((f x) ((pt_quant pt') _ _ e))) ->
+      (forall (e : typD ts nil te), (var_entail var _) ((pt_quant pt) _ _ (fun x => (f x) e)) (((pt_quant pt) _ _ f) e)) ->
+      (forall e e' (ILOps' : ILogicOps (typD ts nil te)) x, (var_entail var' _) e e' -> (var_entail var _) ((f x) e) ((f x) e')) ->
       @valid_arg pt var t ILOps A (te::typs) f ((Some (var', pt'))::args).
 
   Definition valid_env (tus tvs : tenv typ) (xs : list typ) (pt : pull_type) (var : variance) (t : typ) (ILOps : ILogicOps (typD ts nil t)) (typs : list typ)
@@ -168,6 +142,20 @@ End pt_quant_morphisms.
                        forall df, exprD' tus (rev xs ++ tvs) f (fold_right tyArr t typs) = Some df ->
                        forall us vs, @valid_arg pt var t ILOps (HList.hlist _ (rev xs)) typs (fun x => df us (HList.hlist_app x vs)) modes.
   
+
+  Lemma valid_arg_some_inv (pt pt' : pull_type) (var var' : variance) (t te : typ) (ILOps : ILogicOps (typD ts nil t)) (A : Type) 
+    (typs : list typ) (f : A -> typD ts nil te -> typD ts nil (fold_right tyArr t typs)) (modes : list (option (variance * pull_type))) 
+    (H : @valid_arg pt var t ILOps A (te::typs) f ((Some (var', pt'))::modes)) : 
+      (forall B x (e : B -> typD ts nil te) (ILOps' : ILogicOps (typD ts nil te)), 
+             (var_entail var _)  ((pt_quant pt) _ _ (fun y => (f x) (e y))) ((f x) ((pt_quant pt') _ _ e))) /\
+      (forall (e : typD ts nil te), (var_entail var _) ((pt_quant pt) _ _ (fun x => (f x) e)) (((pt_quant pt) _ _ f) e)) /\
+      (forall e e' (ILOps' : ILogicOps (typD ts nil te)) x, (var_entail var' _) e e' -> (var_entail var _) ((f x) e) ((f x) e')).
+  Proof.
+    change (typD ts nil te -> typD ts nil (fold_right tyArr t typs)) with (typD ts nil (fold_right tyArr t (te::typs))) in f.
+    inversion H. subst.
+    apply Eqdep.EqdepTheory.inj_pair2 in H4. subst.
+    intuition.
+  Qed.
 
   Lemma valid_arg_none_inv (pt : pull_type) (var : variance) (t te : typ) (ILOps : ILogicOps (typD ts nil t)) (A : Type) 
     (typs : list typ) (f : A -> typD ts nil te -> typD ts nil (fold_right tyArr t typs)) (modes : list (option (variance * pull_type))) 
@@ -181,41 +169,122 @@ End pt_quant_morphisms.
     intuition.
   Qed.
 
+  Lemma valid_arg_empty (pt : pull_type) (var : variance) (t : typ) (ILOps : ILogicOps (typD ts nil t)) (A : Type) o
+    (f : A -> typD ts nil t) (modes : list (option (variance * pull_type))) 
+    (H : @valid_arg pt var t ILOps A nil f (o::modes)) : False.
+  Proof.
+    change (typD ts nil t) with (typD ts nil (fold_right tyArr t nil)) in f.
+    inversion H.
+  Qed.
+
+  Definition TT := variance -> pull_type -> list typ * expr ilfunc.
+
+  Let T:Type := tenv typ -> tenv typ -> TT.
+  Definition atomic (e : expr ilfunc) : T := fun _ _ _ _ => (nil, e).
+
+  Record pq_env := {
+    pq_env_fun :> ilfunc -> variance -> pull_type -> list (option (variance * pull_type));
+    pq_env_sound : forall f pt var t tus tvs xs (ILOps : ILogicOps (typD ts nil t)) typs, 
+    	typeof_expr tus tvs (Inj f) = Some (fold_right tyArr t typs) ->
+    	valid_env tus tvs xs pt var ILOps typs (Inj f) (pq_env_fun f var pt)
+  }.
+(*
+  Fixpoint typ_empty_mode (t : typ) : list (option (variance * pull_type)) :=
+  	match t with
+  		| tyArr t t' => None::(typ_empty_mode t')
+  		| _          => nil
+    end.
+
+  Program Definition pq_env_empty := {| pq_env_fun := fun f _ _ => match typeof_expr nil nil (Inj f) with 
+                                                                     | Some t => typ_empty_mode t
+                                                                     | None   => nil
+                                                                   end;
+                                        pq_env_sound := _ |}.
+  Next Obligation.
+	unfold valid_env; intros.
+	simpl.
+	remember (typeof_func funcs gs es f). destruct o; [|congruence]. 
+	inv_all; subst.
+	induction typs. simpl.
+	simpl in Heqo.
+	SearchAbout typeof_func.
+	Print typeof_func.
+	destruct f. simpl in *.
+	forward. inv_all; subst. simpl.
+	
+	reflexivity.
+	forward.
+	induction typs. simpl.
+	simpl.
+  
+  Definition env_sound (e : pq_env) tus tvs p := 
+        forall pt var xs t (ILOps : ILogicOps (typD ts nil t)) typs,
+    	typeof_expr tus (rev xs ++ tvs)  = Some (fold_right tyArr t typs) ->
+    	valid_env tus tvs xs pt var ILOps typs (Inj f) (e f var pt).  	
+  *)  
+  Definition pq_var (v : var) : T := atomic (Var v).
+  Definition pq_uvar (u : uvar) : T := atomic (UVar u).
+  Definition pq_inj (s : ilfunc) : T := atomic (Inj s).
+  Definition pq_abs (x : typ) (e : expr ilfunc) (_ : T) : T :=
+    atomic (Abs x e).
+    
+  Fixpoint pq_app_aux (us vs : tenv typ) (ats : list (option (variance * pull_type))) (f : list typ * expr ilfunc) (args : list (expr ilfunc * T)) : list typ * expr ilfunc :=
+  match ats, args with
+  	| Some (var, pt)::ats, (_, t)::args =>
+  	  match f, t us vs var pt with
+  	  	| (xs, f'), (ys, a) => pq_app_aux us vs ats (xs ++ ys, App (lift 0 (length ys) f') (lift (length ys) (length xs) a)) args
+  	  end
+  	| None::ats, (e, _)::args => 
+  	  match f with
+  	    | (xs, f') => pq_app_aux us vs ats (xs, App f' (lift 0 (length xs) e)) args
+  	  end
+  	| _, _ => match f with
+  			  | (xs, f') => (xs, apps f' (map fst args))
+  			  end
+  end.
+  
+  Definition pq_app (e : pq_env) (f : expr ilfunc) (_ : T) (args : list (expr ilfunc * T)) : T :=
+  	fun us vs var pt => 
+  		match f with
+  			| Inj f => pq_app_aux us vs (e f var pt) (nil, Inj f) args
+  			| _     => (nil, apps f (map fst args))
+  		end.
+ 
+  Definition pq_exists (t t_logic : typ) (f : expr ilfunc) (a : T) : T :=
+    fun us vs vm pt =>
+      match pt with
+      	| PExists => let (ts, a) := a us (t :: vs) vm pt in (t::ts, a)
+      	| _       => (nil, App (Inj (ilf_exists t t_logic)) (Abs t f)) 
+      	
+      end.
+
+  Definition pqArgs (e : pq_env) : AppFullFoldArgs ilfunc TT :=
+    @Build_AppFullFoldArgs ilfunc TT pq_var pq_uvar pq_inj pq_abs (pq_app e).
+
   Definition Teval (pt : pull_type) (e : list typ * expr ilfunc) (t : typ) :=
     let (xs, a) := e in add_quants pt t xs a.
         
   Definition TD (pt : pull_type) (t : typ) (e : list typ * expr ilfunc) (us vs : tenv typ) :=
     exprD' us vs (Teval pt e t) t.
-(*
-  Definition Ttype (var : variance) (pt : pull_type) (ts us : tenv typ) (e : TT) (t : typ) :=
-    typeof_expr ts us (Teval pt e t).
 
-  Definition PQtype (var : variance) (pt : pull_type) (e : expr ilfunc) (tt : TT) (us vs : tenv typ) :=
-    match typeof_expr us vs e with
-      | Some t =>
-        match Ttype var pt us vs tt t with
-          | Some t' => t ?[eq] t' = true
-          | None    => True
-        end
-      | None => True
-    end.
-    *)
-Check @TD.
   Definition PQR_aux var pt (t : typ) 
                      (arg : list typ * expr ilfunc)
                      (e : expr ilfunc) (us vs : tenv typ) 
                       :=
    
-    match (TD pt t arg) us vs, exprD' us vs e t, gs t, var with
-      | None, _, _, _ => True
-      | _, _, None, _ => True
-      | Some p, Some q, Some _, CoVariant     => forall us vs, (p us vs) |-- (q us vs)
-      | Some p, Some q, Some _, ContraVariant => forall us vs, (q us vs) |-- (p us vs)
-      | _, _, _, _ => False
+    match (TD pt t arg) us vs, exprD' us vs e t, gs t with
+      | None, _, _ => False
+      | _, _, None => True 
+      | Some p, Some q, Some _ => forall us vs, (var_entail var _) (p us vs) (q us vs)
+      | _, _, _ => False
     end.
     
-  Definition PQR (t : typ) (e : expr ilfunc) (arg : TT) (us vs : tenv typ) :=
-  	forall var pt, PQR_aux var pt t (arg var pt) e us vs.
+  Definition PQR (e : pq_env) (t : typ) (l : expr ilfunc) (arg : TT) (us vs : tenv typ) :=
+  	   forall var pt, 
+  	     forall t' typs, t = fold_right tyArr t' typs ->
+  	     exists modes, forall (ILOps : ILogicOps (typD ts nil t')) xs,
+  	     valid_env us vs xs pt var ILOps typs l modes /\
+  	     PQR_aux var pt t (arg var pt) l us vs.
 
   Lemma ILogic_from_env (t : typ) (i : ILogicOps (typD ts nil t)) (pf : gs t = Some i)
   : @ILogic _ i.
@@ -243,42 +312,74 @@ Check @TD.
   Defined.
   Hint Extern 1 (Reflexive _) => (apply Refl_from_env_lequiv; [ assumption ]) : typeclass_instances.
 
-  Lemma Hatomic tus tvs t e (H : typeof_expr tus tvs e = Some t) :
-    PQR t e (atomic e tus tvs) tus tvs.
+  Lemma HVar (e : pq_env) tus tvs t v (H : typeof_expr tus tvs (Var v) = Some t) :
+    PQR e t (Var v) (atomic (Var v) tus tvs) tus tvs.
   Proof.
+    admit.
+    (*
     unfold atomic, PQR, PQR_aux, TD, Teval; simpl; intros. 
-    forward. 
-    destruct var, pt; forward; simpl in *; forward; inv_all; subst; reflexivity.
+    simpl in *. rewrite H0 in *.
+    exists (map (fun _ => None) typs). intros. split.
+    unfold valid_env; intros.
+    red_exprD; forward; inv_all; subst.
+    
+    Check Eqdep.EqdepTheory.inj_pair2.
+    destruct s.
+    assert (x0 = x). apply Eqdep.EqdepTheory.inj_pair2 in H1.
+    apply Eqdep.EqdepTheory.inj_pair2 in H1. subst.
+    induction typs. simpl. apply ve_nil.
+    simpl in *. apply ve_none. intros. 
+    destruct var, pt. simpl. simpl in *. red_exprD. forward.
+    unfold v
+    split; [intros; inversion H0|]. simpl in *.
+    pose proof (typeof_expr_exprD'_impl RSym_sym tus tvs (Var v) H); destruct H0.
+    destruct var, pt; forward; simpl in *; forward; inv_all; subst; forward; reflexivity.
+    *)
   Qed.
 
-  Lemma Habs 
-  : forall tus tvs t t' e e_res,
-      typeof_expr tus tvs (Abs t e) = Some (tyArr t t') ->
-      @PQR t' e (e_res tus (t :: tvs)) tus (t :: tvs) ->
-      @PQR (tyArr t t') (Abs t e) (pq_abs t e e_res tus tvs) tus tvs.
+  Lemma Habs (e : pq_env) 
+  : forall tus tvs t t' f e_res,
+      typeof_expr tus tvs (Abs t f) = Some (tyArr t t') ->
+      @PQR e t' f (e_res tus (t :: tvs)) tus (t :: tvs) ->
+      @PQR e (tyArr t t') (Abs t f) (pq_abs t f e_res tus tvs) tus tvs.
   Proof.
-    intros; apply Hatomic; assumption.
+    admit.
+    (*
+    intros.
+    unfold atomic, PQR, PQR_aux, TD, Teval; simpl; intros.
+    split; [intros; inversion H1|]. simpl in *.
+    pose proof (typeof_expr_exprD'_impl RSym_sym tus tvs (Abs t f) H); destruct H1.
+    destruct var, pt; forward; simpl in *; forward; inv_all; subst; forward; simpl in *.
+    specialize (gsOk (tyArr t t')). forward. inv_all; subst. simpl in *.
+    admit. admit. admit. admit. (* I have no idea why this doesn't work *)
+    *)
   Qed.
 
   Lemma Hex 
-  : forall (tus tvs : tenv typ) t t_logic e (e_res : T),
-      typeof_expr tus tvs (App (Inj (ilf_exists t t_logic)) (Abs t e)) = Some t_logic ->
-      PQR t_logic e (e_res tus (t :: tvs)) tus (t :: tvs) ->
-      PQR t_logic
-          (App (Inj (ilf_exists t t_logic)) (Abs t e))
-          (@pq_exists t t_logic e e_res tus tvs) tus tvs.
+  : forall (e : pq_env) (tus tvs : tenv typ) t t_logic f (e_res : T),
+      typeof_expr tus tvs (App (Inj (ilf_exists t t_logic)) (Abs t f)) = Some t_logic ->
+      PQR e t_logic f (e_res tus (t :: tvs)) tus (t :: tvs) ->
+      PQR e t_logic
+          (App (Inj (ilf_exists t t_logic)) (Abs t f))
+          (@pq_exists t t_logic f e_res tus tvs) tus tvs.
   Proof.
+    admit.
+    (*
     unfold PQR; intros. 
     specialize (H0 var pt).
+    split; [intros; inversion H1|].
     destruct pt; simpl in *; unfold PQR_aux, TD, Teval in *; simpl in *.
-    + red_exprD; forward; inv_all; subst. 
+    + red_exprD; forward; inv_all; subst.  
+      red_exprD; forward; inv_all; subst.
+      rewrite typ_cast_typ_refl.
       destruct var; intros; uip_all; reflexivity.
-    + red_exprD; forward; simpl in *; inv_all; simpl in *; subst. unfold add_quant in H5; simpl in H5.
-      red_exprD; forward; simpl in *; inv_all; simpl in *. revert H10. subst.  intros. destruct H3; subst.
+    + red_exprD; forward; simpl in *; inv_all; simpl in *; subst. unfold add_quant; simpl. 
+      red_exprD; forward; simpl in *; inv_all; simpl in *. subst.  intros. destruct H4; subst.
       red_exprD; forward; simpl in *; inv_all; simpl in *; subst.
       red_exprD; forward; inv_all; simpl in *; subst.
-      uip_all. subst.
-      destruct var; intros; setoid_rewrite H8; reflexivity.
+      uip_all. subst. destruct H3 as [_ H3].
+      destruct var; intros; setoid_rewrite H3; reflexivity.
+      *)
   Qed.
 
   Lemma typeof_expr_apps uvs vvs e lst (H: typeof_expr uvs vvs e = None) :
@@ -303,80 +404,103 @@ Check @TD.
     destruct (pq_env i pt vars); [reflexivity|]. simpl. destruct o; try reflexivity.
     destruct p; reflexivity.
   Qed.
-
+(*
   Lemma pqapp_cons_cases pq_env a ats l l_res tus tvs pt vars xs e 
   	(H : pq_app pq_env l l_res (a :: ats) tus tvs pt vars = (xs, e)) :
   	(xs = nil /\ e = l) \/
   	(exists f, l = Inj f /\ pq_app_aux tus tvs (pq_env f pt vars) (nil, Inj f) (a :: ats) = (xs, e)).
   Proof.
     destruct l; simpl in *; inv_all; subst; try (left; split; reflexivity).
-    right. exists i. firstorder.
-Qed.
-  (*
-  Lemma PQR_app_inj pt vars t pq_env l xs l_res tus tvs 
-    (H : forall f, l = Inj f -> PQR pt vars t l (pq_app pq_env l l_res xs tus tvs) tus tvs) :
-  	PQR pt vars t l (pq_app pq_env l l_res xs tus tvs) tus tvs.
-  Proof.
-    destruct l; try (clear H; unfold PQR, TD, Teval, add_quant; simpl; forward; destruct vars; forward; inv_all; subst; destruct pt; reflexivity).
-    eapply H. reflexivity.
+    right. exists v. firstorder.
   Qed.
 *)
-  Lemma PQR_app_nil t pq_env l l_res tus tvs :
-  	PQR t l (pq_app pq_env l l_res nil tus tvs) tus tvs.
+  Lemma PQR_app_nil t pq_env l l_res tus tvs 
+    (H : typeof_expr tus tvs l = Some t) :
+  	PQR pq_env t l (pq_app pq_env l l_res nil tus tvs) tus tvs.
   Proof.
+    admit.
+    (*
+    apply typeof_expr_exprD' in H. destruct H. 
     unfold PQR, PQR_aux, TD, Teval, add_quant; intros.
-    simpl. forward.
-    rewrite pqapp_nil in H. inv_all; subst; simpl in *.
+    simpl. forward. inv_all; subst. forward.
+    rewrite pqapp_nil in H0. inv_all; subst; simpl in *.
     destruct var, pt; forward; inv_all; subst; reflexivity.
+    *)
   Qed.
 
- Lemma PQR_atomic vars pt t xs f tus tvs : PQR_aux vars pt t (xs, f) (add_quants pt t xs f) tus tvs.
- Proof.
-   unfold PQR_aux, TD, Teval.
-   forward. destruct vars; intros; reflexivity.
- Qed.
 
-     Lemma lift_app (sym : Type) x y (f e : expr sym) :
-     	lift x y (App f e) = App (lift x y f) (lift x y e).
-     Proof.
-       repeat rewrite lift_lift'; simpl; reflexivity.
-     Qed.
+  Lemma add_quants_typeof_expr tus tvs xs f pt t (ILOps : ILogicOps (typD ts nil t)) (HIL : gs t = Some ILOps) :
+  	typeof_expr tus (rev xs ++ tvs) f = Some t <-> typeof_expr tus tvs (add_quants pt t xs f) = Some t.
+  Proof.
+    generalize dependent tvs. generalize dependent f.
+    induction xs; intros.
+    + simpl in *; reflexivity.
+    + simpl in *. rewrite <- app_assoc. simpl in *.
+      rewrite IHxs; destruct pt; simpl in *; forward; inv_all; subst; simpl; forward.
+  Qed.
 
- Lemma lift_apps (sym : Type) x y (f : expr sym) args :
- 	lift x y (apps f args) = apps (lift x y f) (map (lift x y) args).
- Proof.
-   generalize dependent f. induction args; intros.
-   + simpl. reflexivity.
-   + simpl. rewrite IHargs, lift_app; reflexivity.
- Qed.
+  Lemma PQR_atomic vars pt t xs f tus tvs (ILOps : ILogicOps (typD ts nil t)) (HIL : gs t = Some ILOps)
+   (H : typeof_expr tus (rev xs ++ tvs) f = Some t) : 
+   PQR_aux vars pt t (xs, f) (add_quants pt t xs f) tus tvs.
+  Proof.
+    rewrite add_quants_typeof_expr with (pt := pt) in H; [|eassumption].
+    apply typeof_expr_exprD' in H. destruct H.
+    unfold PQR_aux, TD, Teval.
+    forward. destruct vars; intros; reflexivity.
+  Qed.
 
-       	  Lemma PQR_atom tus tvs vars pt xs t f g (ILOps : ILogicOps (typD ts nil t)) (Hgs : gs t = Some ILOps)
-       	    (Hg : typeof_expr tus tvs g = Some t)
-       	    (Heq : forall df dg, exprD' tus tvs (add_quants pt t xs f) t = Some df -> exprD' tus tvs g t = Some dg -> forall us vs, df us vs -|- dg us vs) :
-       	    PQR_aux vars pt t (xs, f) g tus tvs.
-       	  Proof.
-       	    unfold PQR_aux, TD, Teval.
-       	    apply typeof_expr_exprD'_impl in Hg. destruct Hg.
-        	    forward; inv_all; subst.
-       	    destruct vars; intros.
-       	    rewrite Heq; reflexivity.
-       	    rewrite <- Heq; reflexivity.
-		  Qed.
+  Lemma lift_app (sym : Type) x y (f e : expr sym) :
+  	lift x y (App f e) = App (lift x y f) (lift x y e).
+  Proof.
+    repeat rewrite lift_lift'; simpl; reflexivity.
+  Qed.
 
-    Lemma PQR_typeof vars pt t xs f g tus tvs (ILOps : ILogicOps (typD ts nil t)) (Hgs : gs t = Some ILOps)
-        (Hf : typeof_expr tus tvs (add_quants pt t xs f) = Some t)
+  Lemma lift_apps (sym : Type) x y (f : expr sym) args :
+  	lift x y (apps f args) = apps (lift x y f) (map (lift x y) args).
+  Proof.
+    generalize dependent f. induction args; intros.
+    + simpl. reflexivity.
+    + simpl. rewrite IHargs, lift_app; reflexivity.
+  Qed.
+
+  Lemma PQR_atom tus tvs vars pt xs t f g (ILOps : ILogicOps (typD ts nil t)) (Hgs : gs t = Some ILOps)
+    (Hf : typeof_expr tus (rev xs ++ tvs) f = Some t)
+    (Hg : typeof_expr tus tvs g = Some t)
+    (Heq : forall df dg, exprD' tus tvs (add_quants pt t xs f) t = Some df -> exprD' tus tvs g t = Some dg -> forall us vs, df us vs -|- dg us vs) :
+    PQR_aux vars pt t (xs, f) g tus tvs.
+  Proof.
+    unfold PQR_aux, TD, Teval.
+    apply typeof_expr_exprD' in Hg. destruct Hg.
+    eapply add_quants_typeof_expr with (pt := pt) in Hf; [|eassumption].
+    apply typeof_expr_exprD' in Hf. destruct Hf.
+	    forward; inv_all; subst.
+	rewrite Heq; reflexivity. 
+  Qed.
+
+	Lemma PQR_typeof vars pt t xs f g tus tvs (ILOps : ILogicOps (typD ts nil t)) (Hgs : gs t = Some ILOps)
+	    (Hf : typeof_expr tus tvs (add_quants pt t xs f) = Some t)
+	 	(H : PQR_aux vars pt t (xs, f) g tus tvs) :
+	 	typeof_expr tus tvs g = Some t.
+	 Proof.
+	   	unfold PQR_aux, TD, Teval in H. 
+	   	apply typeof_expr_exprD'_impl in Hf.
+	    destruct Hf. forward. inv_all; subst.
+	    eapply ExprD3.EXPR_DENOTE_core.exprD'_typeof; eassumption.
+	Qed.
+
+    Lemma PQR_typeof2 vars pt t xs f g tus tvs (ILOps : ILogicOps (typD ts nil t)) (Hgs : gs t = Some ILOps)
+        (Hg : typeof_expr tus tvs g = Some t)
      	(H : PQR_aux vars pt t (xs, f) g tus tvs) :
-     	typeof_expr tus tvs g = Some t.
+        typeof_expr tus tvs (add_quants pt t xs f) = Some t.
      Proof.
        	unfold PQR_aux, TD, Teval in H. 
-       	apply typeof_expr_exprD'_impl in Hf.
-        destruct Hf. forward. inv_all; subst.
-        SearchAbout typeof_expr exprD'.
-        eapply ExprD3.EXPR_DENOTE_core.exprD'_typeof; eassumption.
-Qed.
+       	apply typeof_expr_exprD'_impl in Hg.
+        destruct Hg. forward. inv_all; subst.
+        eapply ExprD3.EXPR_DENOTE_core.exprD'_typeof. eassumption.
+    Qed.
 
   
- Lemma exprD'_add_quants_cons_Some (pt : pull_type) (Ty : typ) (IL_Ty : ILogicOps (typD ts nil Ty))
+  Lemma exprD'_add_quants_cons_Some (pt : pull_type) (Ty : typ) (IL_Ty : ILogicOps (typD ts nil Ty))
         (_ : gs Ty = Some IL_Ty)
   : forall tus tvs tm a b x,
       exprD' tus tvs (add_quants pt Ty (a :: b) tm) Ty = Some x ->
@@ -417,7 +541,6 @@ Qed.
         inv_all. subst.
         reflexivity. }
    Qed.
-     Require Import ExtLib.Data.HList.
    
   Lemma exists_hlist_app (Ty : typ) (ILO_Ty : ILogicOps (typD ts nil Ty))
         (IL_Ty : ILogic (typD ts nil Ty))
@@ -496,7 +619,7 @@ Qed.
       apply lforallR; intros.
       eapply lforallL; eauto.
       eapply lforallL; eauto. eapply H. }
-     Qed.
+   Qed.
      
    Lemma pt_iff_2 (Ty : Type) (ILO_Ty : ILogicOps Ty) pt
         (IL_Ty : ILogic Ty)
@@ -546,7 +669,7 @@ Qed.
       destruct IHxs.
       { clear.
         generalize dependent ((rev xs ++ a :: nil) ++ tvs).
-        intros; subst. (** eta **) reflexivity. }
+        intros; subst. (** eta *) reflexivity. }
       { destruct H2. destruct pt; simpl in *;
         unfold add_quant; simpl.
 	    + red_exprD.
@@ -748,2444 +871,226 @@ Qed.
     rewrite <- (app_nil_r a) in H0.
     apply exprD'_add_quants_app_Some in H0; eauto.
   Qed.
- 
-     
-    			  
-    
-   
-   
+
+ Lemma PQR_aux_rewrite tus tvs e1 e2 t vars pt e3 (ILOps : ILogicOps (typD ts nil t)) (Hgs : gs t = Some ILOps) (IL : ILogic (typD ts nil t))
+    (H : forall de2, exprD' tus tvs e2 t = Some de2 -> exists de3, exprD' tus tvs e3 t = Some de3 /\ forall us vs, (var_entail vars _) (de2 us vs) (de3 us vs))
+ 	(He2 : PQR_aux vars pt t e1 e2 tus tvs) :
+ 	PQR_aux vars pt t e1 e3 tus tvs.
+ Proof.
+   	unfold PQR_aux, TD, Teval in *.
+   	forward; inv_all; subst.
+   	specialize (H2 t1 eq_refl).
+   	destruct H2. destruct H0.
+   	forward; inv_all; subst.
+   	rewrite He2, H2; reflexivity.
+ Qed.
+
+     Lemma apps_rewrite tus tvs e1 e2 rs t dea1 (ILOps : ILogicOps (typD ts nil t)) vars
+        (H : exprD' tus tvs (apps e1 rs) t = Some dea1) 
+        (He: forall typs de1, exprD' tus tvs e1 (fold_right tyArr t typs) = Some de1 -> 
+        	                exists de2, exprD' tus tvs e2 (fold_right tyArr t typs) = Some de2 /\ forall us vs, (var_entail vars _ ) (de1 us vs) (de2 us vs)) :
+        exists dea2, exprD' tus tvs (apps e2 rs) t = Some dea2 /\ forall us vs, (var_entail vars _) (dea1 us vs) (dea2 us vs).
+     Proof.
+       generalize dependent e1; generalize dependent e2; induction rs; simpl in *; intros.
+       + specialize (He nil). apply He. simpl. apply H.
+      + eapply IHrs; [eassumption |].
+         intros.
+         red_exprD; forward; inv_all; subst. clear IHrs.
+         specialize (He (t1::typs) _ H2).
+         destruct He as [de2 [He1 He2]].
+         simpl in *.
+         SearchAbout exprD' typeof_expr.
+         assert (typeof_expr tus tvs e2 = Some (tyArr t1 (fold_right tyArr t typs))) by admit.
+         forward; inv_all; subst.
+         forward; inv_all; subst.
+         rewrite typ_cast_typ_refl.
+         eexists. split; [reflexivity|]. intros.
+         simpl. 
+         assert ((var_entail vars _) (t3 us vs) (de2 us vs)). apply He2.
+         Local Transparent ILFun_Ops.
+         destruct vars; apply H5.
+    Qed.
 
  
   Lemma Happ pq_env
   : forall tus tvs l (l_res : T) rs t ts,
       typeof_expr tus tvs (apps l (map fst rs)) = Some t ->
       let ft := fold_right tyArr t ts in
-      PQR ft l (l_res tus tvs) tus tvs ->
+      PQR pq_env ft l (l_res tus tvs) tus tvs ->
       Forall2 (fun t x =>
                     typeof_expr tus tvs (fst x) = Some t
-                 /\ PQR t (fst x) (snd x tus tvs) tus tvs)
+                 /\ PQR pq_env t (fst x) (snd x tus tvs) tus tvs)
               ts rs ->
-      PQR t (apps l (map fst rs)) (pq_app pq_env l l_res rs tus tvs) tus tvs.
+      PQR pq_env t (apps l (map fst rs)) (pq_app pq_env l l_res rs tus tvs) tus tvs.
    Proof.
      intros.
      intros vars pt. simpl.
      assert (exists ILOps, (gs t) = Some ILOps) by admit. destruct H2.
-     assert (exists f, l = Inj f) by admit. destruct H3 as [f H3]. subst.
-     unfold pq_app.
-     specialize (H0 vars pt). 
-     assert (typeof_expr tus tvs (Inj f) = Some ft).
-     clear H0. generalize dependent (Inj f). generalize dependent ts0.
-     induction rs; simpl in *; intros.
-	 inversion H1. simpl. apply H.
-	 inversion H1; subst. simpl.
-	 specialize (IHrs _ H6 _ H).
-	 destruct H5 as [H5 _].
-	 SearchAbout typeof_expr.
-	 simpl in *. forward; inv_all; subst. simpl in *.
-	 f_equal.
-	 SearchAbout type_of_apply.
-	 unfold type_of_apply in IHrs.
-	 destruct t0; try congruence.
-	 forward.
-	 (*
-	 Lemma exprD'_pull_empty tus tvs pt xs t f e df (ILOps : ILogicOps (typD ts nil t)) (IL : ILogic (typD ts nil t)) te
-	   (He : typeof_expr tus tvs e = Some te)
-	   (Hf : typeof_expr tus (rev xs ++ tvs) f = Some (tyArr te t))
-	   (H : exprD' tus tvs (add_quants pt t xs (App f (lift 0 (length xs) e))) t = Some df) :
-	   exists df', exprD' tus tvs (App (add_quants pt (tyArr te t) xs f) e) t = Some df' /\ forall us vs, df us vs -|- df' us vs.
-	 Proof.
-	   apply exprD'_add_quants_all_Some in H.
-	   destruct H as [de [H1 H2]].
-	   red_exprD; forward; inv_all; simpl in *. clear H7. revert H2. subst. intros.
-	 Lemma add_quants_typeof_expr tus tvs xs f pt t (ILOps : ILogicOps (typD ts nil t)) (HIL : gs t = Some ILOps) :
-	 	typeof_expr tus (rev xs ++ tvs) f = Some t <-> typeof_expr tus tvs (add_quants pt t xs f) = Some t.
-	 Proof.
-	   generalize dependent tvs. generalize dependent f.
-	   induction xs; intros.
-	   + simpl in *; reflexivity.
-	   + simpl in *. rewrite <- app_assoc. simpl in *.
-	     rewrite IHxs; destruct pt; simpl in *; forward; inv_all; subst; simpl; forward.
-	 Qed.
-	   assert (gs (tyArr te t) = Some (@ILFun_Ops (typD ts nil te) (typD ts nil t) ILOps)) by admit.
-	   rewrite add_quants_typeof_expr with (pt := pt) in H0; [|eassumption].
-	   setoid_rewrite H0.
-	   pose proof (@exprD'_add_quants_rev_Some (tyArr te t)).
-	   specialize (H4 (@ILFun_Ops (typD ts nil te) (typD ts nil t) ILOps) pt H tus xs tvs _ _ H1).
-	   destruct H4 as [? [? ?]].
-	   rewrite H4.
-	   rewrite typ_cast_typ_refl.
-	   pose proof (exprD'_lift RSym_sym tus nil (rev xs) tvs e te).
-	   simpl in H6. rewrite rev_length in H6. forward.
-	   eexists.
-	   split. reflexivity. intros. rewrite H2.
-	   inv_all; subst.
-	   
-	   inv_all; subst.
-	   rewrite <- H8.
-	    rewrite H5.
-	   rewrite H3 in H6.
-	   simpl in H6. forward.
-	   edestruct H as [? ?].
-	   edestruct H5.
-	   erewrite H6.
-	   destruct H as [? [? ?]].
-	   Check ILFun_Ops.
-	   apply exprD'_add_quants_rev_Some in H1.
-	 apply add_quants_typeof_expr in H3.
-	     simpl. forward. destruct H2; [congruence|].
-	     
-	    rewrite <- app_assoc. simpl.
-	     destruct pt; simpl. 
-	     forward; inv_all; subst.
-	     split; intros. 
-	     rewrite <- IHxs.
-	     rewrite <- IHxs.
-	     rewrite H.
-	     forward; inv_all; subst.
-	     simpl.
-	     forward.
-	     rewrite <- IHxs in H1. rewrite H1.
-	     rewrite IHxs. rewrite <- IHxs in H1.
-	     simpl. forward. inv_all; subst.
-	     destruct H2; [congruence|].
-	     rewrite <- IHxs. rewrite H1. c
-	   rewrite IHxs.
-	     destruct pt. simpl. forward; simpl in *. inv_all; subst.
-	     remember (typ_eqb a a). destruct b.
-	     simpl in *. unfold add_quants in H1. simpl in H1. simpl in *.
-	     unfold add_quant in H1. simpl in *.
-	     SearchAbout typ_eqb.
-	     rewrite refl_typ_eqb.
-	     inv_all; subst. 
-	     unfold type_of_apply.
-	   simpl in *; intros. subst.
-	   pose proof (exprD'_lift RSym_sym tus nil (rev xs) tvs).
-	   simpl in H. rewrite rev_length in H. forward.
-	   revert de H1 H2.
-	   replace (rev xs ++ tvs) with (nil ++ rev xs ++ tvs) by reflexivity.
-	   red_exprD.
-	   admit.
-    Qed.
-    (*
-	   generalize dependent tvs; generalize dependent e; induction xs; intros.
-	   + simpl in *. exists df. split; [|reflexivity].
-	     destruct pt; simpl in *; assumption.
-	   + simpl in *.
-	     destruct pt.
-	     unfold add_quant in *. simpl in *.
-	     red_exprD; forward; simpl in *; inv_all. clear H7. revert H4. subst. intros.
-	     red_exprD; forward; simpl in *; inv_all; subst.
-	     red_exprD; forward; simpl in *; inv_all; subst.
-         red_exprD; forward; simpl in *; inv_all; subst.
-         replace (S (length xs)) with (length xs + 1) in H2 by omega.
-         rewrite <- lift_lift', <- lift_lift in H2.
-         rewrite <- app_assoc in Hf. simpl in Hf.
-         assert (typeof_expr tus (nil++(a::nil)++tvs) (lift (length (@nil typ)) (length (a::nil)) e) = Some te).
-         rewrite typeof_expr_lift. simpl. assumption.
-         simpl in *. rewrite <- lift_lift' in H0.
-         specialize (IHxs _ _ _ H0 Hf H2).
-         destruct IHxs as [df [H4 H5]].
-         Check HList.hlist_tl.
-         exists (fun us vs => Forall x : typD ts nil a, df us (HList.Hcons x vs)).
-         red_exprD; forward; simpl in *; inv_all; subst.
-         assert (typ_eqb t (tyArr t2 t) = true). admit. forward.
-         red_exprD; forward; simpl in *; inv_all; revert H1. subst.
-         red_exprD; forward; simpl in *; inv_all; subst.
-         forward.
-         red_exprD; forward; simpl in *; inv_all; subst.
-         assert (typ_eqb t (tyArr t2 t) = false) by admit.
-         forward.
-         *)
-     *)
+     specialize (H0 vars pt).
+     assert (typeof_expr tus tvs l = Some ft). {
+     	clear H0. generalize dependent l; generalize dependent ts0.
+     	induction rs; simpl in *; intros; inversion H1; simpl.
+     	+ apply H.
+     	+ specialize (IHrs _ H6 _ H).
+     	  destruct H5 as [H5 _].
+     	  simpl in *; forward; inv_all; subst; simpl in *.
+     	  f_equal. unfold type_of_apply in IHrs.
+     	  destruct t0; try congruence.
+     	  forward.
+     }
 
-     Lemma Happ_aux tus tvs pt vars f rs t modes xs typs (ILOps : ILogicOps (typD ts nil t)) (IL : ILogic (typD ts nil t)) (Hgs : gs t = Some ILOps)
+     intros.  
+     specialize (H0 t ts0 eq_refl).
+     destruct H0 as [H0 H5].
+     exists nil. intros.
+     split; [admit|].
+     destruct l. simpl.
+     admit.
+     replace (apps (Inj i) (map fst rs)) with (apps (add_quants pt (fold_right tyArr t ts0) nil (Inj i)) (map fst rs)).
+
+
+     Lemma Happ_aux pq_env tus tvs pt vars f rs t modes xs typs (ILOps : ILogicOps (typD ts nil t)) (IL : ILogic (typD ts nil t)) (Hgs : gs t = Some ILOps)
         (Hf : typeof_expr tus (rev xs ++ tvs) f = Some (fold_right tyArr t typs))
         (Hrs : Forall2
 		       (fun (t : typ) (x : expr ilfunc * (tenv typ -> tenv typ -> TT)) =>
 		        typeof_expr tus tvs (fst x) = Some t /\
-		        PQR t (fst x) (snd x tus tvs) tus tvs) typs rs)
+		        PQR pq_env t (fst x) (snd x tus tvs) tus tvs) typs rs)
         (Henv : @valid_env tus tvs xs pt vars t ILOps typs f modes) :
      	PQR_aux vars pt t (pq_app_aux tus tvs modes (xs, f) rs)
      	                  (apps (add_quants pt (fold_right tyArr t typs) xs f) (map fst rs)) tus tvs.
      Proof.
-        generalize dependent typs. generalize dependent f.
+        generalize dependent typs. generalize dependent f. generalize dependent modes. generalize dependent xs.
        	induction rs; intros.
-       	+ admit.
+       	+ inversion Hrs; subst. destruct modes; simpl in *. 
+       	  * unfold PQR_aux, TD, Teval. simpl. forward; inv_all; subst.
+       	    rewrite add_quants_typeof_expr with (pt := pt) in Hf; [|eassumption].
+       	    apply typeof_expr_exprD' in Hf. destruct Hf. forward.
+       	    destruct vars; reflexivity.
+       	  * unfold valid_env in Henv. simpl in *.
+       	    pose proof Hf.
+       	    rewrite add_quants_typeof_expr with (pt := pt) in Hf; [|eassumption].
+       	    apply typeof_expr_exprD' in Hf. destruct Hf. forward.
+       	    apply typeof_expr_exprD'_impl in H. destruct H.
+       	    specialize (Henv _ H).
+       	    destruct o. destruct p. unfold PQR_aux, TD, Teval. forward. inv_all; subst.
+       	    destruct vars; intros; reflexivity.
+       	    unfold PQR_aux, TD, Teval; forward. destruct vars; reflexivity.
        	+ destruct typs; [inversion Hrs|].
        	  destruct modes; [admit|].
        	  inversion Hrs; clear Hrs; subst. destruct H2.
-       	  destruct o; simpl. destruct p, a; simpl.
-       	  admit. destruct a. simpl.
-       	    
-     Lemma PQR_aux_rewrite tus tvs e1 e2 t vars pt e3 (ILOps : ILogicOps (typD ts nil t)) (Hgs : gs t = Some ILOps) (IL : ILogic (typD ts nil t))
-        (H : forall de2, exprD' tus tvs e2 t = Some de2 -> exists de3, exprD' tus tvs e3 t = Some de3 /\ forall us vs, de2 us vs -|- de3 us vs)
-     	(He2 : PQR_aux vars pt t e1 e2 tus tvs) :
-     	PQR_aux vars pt t e1 e3 tus tvs.
-     Proof.
-       	unfold PQR_aux, TD, Teval in *.
-       	forward; inv_all; subst.
-       	specialize (H2 t1 eq_refl).
-       	destruct H2. destruct H0.
-       	forward; inv_all; subst.
-       	destruct vars; intros.
-       	+ rewrite He2, H2; reflexivity.
-       	+ rewrite <- He2, H2; reflexivity.
-     Qed.
-       
-     
-       
-     Lemma apps_rewrite tus tvs e1 e2 rs t dea1 (ILOps : ILogicOps (typD ts nil t))
-        (He: forall ts de1, exprD' tus tvs e1 (fold_right tyArr t ts) = Some de1 -> 
-        	                exists de2, exprD' tus tvs e2 (fold_right tyArr t ts) = Some de2 /\ forall us vs, de1 us vs -|- de2 us vs)
-        (H : exprD' tus tvs (apps e1 rs) t = Some dea1) :
-        exists dea2, exprD' tus tvs (apps e2 rs) t = Some dea2 /\ forall us vs, dea1 us vs -|- dea2 us vs.
-     Proof.
-       generalize dependent e1; generalize dependent e2; induction rs; simpl in *; intros.
-       + specialize (He nil). simpl in *. apply He. apply H.
-       + eapply IHrs; [|eassumption].
-         intros.
-         red_exprD; forward; inv_all; subst. clear IHrs.
-         specialize (He (t1::ts0) _ H2).
-         destruct He as [de2 [He1 He2]].
-         simpl in *.
-         SearchAbout exprD' typeof_expr.
-         assert (typeof_expr tus tvs e2 = Some (tyArr t1 (fold_right tyArr t ts0))) by admit.
-         forward; inv_all; subst.
-         forward; inv_all; subst.
-         rewrite typ_cast_typ_refl.
-         eexists. split; [reflexivity|]. intros.
-         simpl. 
-         assert (@lequiv (typD ts nil (fold_right tyArr t (t1::ts0))) _ (t3 us vs) (de2 us vs)). apply He2.
-         Local Transparent ILFun_Ops.
-         split; apply H5.
-    Qed.
+       	  destruct o; simpl in *. 
+       	  * destruct p, a; simpl in *.
+       	    unfold PQR in H0. specialize (H0 v p).
+       	    forward. 
+       	    apply (PQR_aux_rewrite (e2 := apps (add_quants pt (fold_right tyArr t typs) (xs ++ l) (App (lift 0 (length l) f) (lift (length l) (length xs) e0))) (map fst rs))); [assumption | assumption | |]. 
+            intros.
+            apply (apps_rewrite (e1 := add_quants pt (fold_right tyArr t typs) (xs ++ l) (App (lift 0 (length l) f) (lift (length l) (length xs) e0)))); [assumption|].
+            intros.
+		    assert (gs (fold_right tyArr t typs) = Some _) by admit.
+		    assert (typs = typs0) by admit; subst. simpl in *.
+            pose proof (exprD'_add_quants_app_Some H5 H3).
+            destruct H5 as [de3 [Hde3 Heq]].
+            red_exprD; forward; inv_all; subst; intros.
+		    destruct H6 as [? [? ?]].
+		    replace l with (l ++ nil) in H5 by (apply app_nil_r).
+            assert (gs ((fold_right tyArr t typs0)) = Some _) by admit. simpl in H6.
+		    pose proof (exprD'_add_quants_app_Some H7 H5).
+		    destruct H8 as [? [? ?]]. rewrite app_nil_r in H8. simpl in H8.
+		    red_exprD; forward; inv_all; subst.
+		    pose proof (typeof_expr_lift RSym_sym tus nil (rev l) (rev xs ++ tvs) f); simpl in H8. 
+		    rewrite rev_length in H8. rewrite H8 in H10. rewrite H10 in Hf. inv_all; revert H9; subst; intros. 
+		    rewrite add_quants_typeof_expr with (pt := pt) in H10.
+		    forward; inv_all; subst.
+		    pose proof (exprD'_lift RSym_sym tus nil (rev l) (rev xs ++ tvs) f (tyArr t0 (fold_right tyArr t typs0))).
+		    simpl in H10. rewrite rev_length in H10. forward.
+            assert (gs ((fold_right tyArr t (t0::typs0))) = Some _) by admit. simpl in H17.
+		    pose proof (@exprD'_add_quants_rev_Some (tyArr t0 (fold_right tyArr t typs0)) _ pt H17 tus xs tvs _ _ H15).
+		    destruct H18 as [? [? ?]].
+		    forward. inv_all; subst.
+		    pose proof (exprD'_lift RSym_sym tus (rev l) (rev xs) tvs e0 t0).
+		    do 2 rewrite rev_length in H11. forward; inv_all; subst.
+		    unfold PQR_aux, TD, Teval in H1.
+		    forward; inv_all; subst.
+		    forward; inv_all; subst.
+		    assert (exists ILOps', gs t0 = Some ILOps') by admit. destruct H12.
+		    forward; inv_all; subst.
+		    rewrite typ_cast_typ_refl.
+		    specialize (H12 t0 nil eq_refl). destruct H12. specialize (H12 x1 nil). destruct H12.
+		    forward; inv_all; subst.
+		    exists (fun us vs => (x0 us vs) (t7 us vs)). split. reflexivity.
+		    intros.
+		    unfold valid_env in Henv.
+		    specialize (Henv _ H15 us vs).
+		    apply valid_arg_some_inv in Henv. destruct Henv as [? [? ?]].
+		    rewrite H6. setoid_rewrite H9. 
+		    specialize (H16 us HList.Hnil). simpl in H16.
+		    assert (var_entail vars (ILogic_Ops_fold_fun (t:=t) ILOps typs0) 
+  (pt_quant pt (ILogic_Ops_fold_fun (t:=t) ILOps typs0)
+     (fun v0 : hlist (typD ts nil) (rev xs) =>
+      pt_quant pt (ILogic_Ops_fold_fun (t:=t) ILOps typs0)
+        (fun v1 : hlist (typD ts nil) (rev l) =>
+         t5 us (hlist_app v1 (hlist_app v0 vs))
+           (t6 us (hlist_app v1 (hlist_app v0 vs)))))) (x0 us vs (t7 us vs)) =
+var_entail vars (ILogic_Ops_fold_fun (t:=t) ILOps typs0)
+  (pt_quant pt (ILogic_Ops_fold_fun (t:=t) ILOps typs0)
+     (fun v0 : hlist (typD ts nil) (rev xs) =>
+      pt_quant pt (ILogic_Ops_fold_fun (t:=t) ILOps typs0)
+        (fun v1 : hlist (typD ts nil) (rev l) =>
+         t3 us (hlist_app v0 vs) (t4 us (hlist_app v1 vs)))))
+  (x0 us vs (t7 us vs))).
+           f_equal. f_equal.
+           Require Import FunctionalExtensionality.
+            apply functional_extensionality; intros.
+            apply f_equal.
+            apply functional_extensionality.
+            intros.
+            rewrite H16, H21; reflexivity. 
+            Lemma blarf (P Q : Prop) (HPQ : P = Q) (H : Q) : P. rewrite HPQ. assumption. Qed.
 
-    apply (PQR_aux_rewrite (e2 := apps (add_quants pt (fold_right tyArr t typs) xs (App f (lift 0 (length xs) e))) (map fst rs))).
-    assumption.
-    assumption.
-    intros.
-    apply (apps_rewrite (e1 := add_quants pt (fold_right tyArr t typs) xs (App f (lift 0 (length xs) e)))); [|assumption].
-    intros.
-    replace xs with (xs ++ nil) in H2.
-    Check exprD'_add_quants_app_Some.
-    assert (gs (fold_right tyArr t typs) = Some _) by admit.
-    assert (ts0 = typs) by admit; subst. simpl in *.
-    pose proof (exprD'_add_quants_app_Some H3 H2).
-    simpl in H5.
-    destruct H5 as [de3 [Hde3 Heq]].
-    red_exprD; forward; inv_all; revert Heq; subst; intros.
-    
-     Lemma add_quants_typeof_expr tus tvs xs f pt t (ILOps : ILogicOps (typD ts nil t)) (HIL : gs t = Some ILOps) :
-	 	typeof_expr tus (rev xs ++ tvs) f = Some t <-> typeof_expr tus tvs (add_quants pt t xs f) = Some t.
-	 Proof.
-	   generalize dependent tvs. generalize dependent f.
-	   induction xs; intros.
-	   + simpl in *; reflexivity.
-	   + simpl in *. rewrite <- app_assoc. simpl in *.
-	     rewrite IHxs; destruct pt; simpl in *; forward; inv_all; subst; simpl; forward.
-	 Qed.
-    assert (gs ((fold_right tyArr t (t0::typs))) = Some _) by admit. simpl in H5.
-    rewrite add_quants_typeof_expr with (pt := pt) in H6; [|eassumption].
-    forward. inv_all; subst.
-    revert Heq. uip_all'. intros.
-    pose proof (@exprD'_add_quants_rev_Some (tyArr t0 (fold_right tyArr t typs)) _ pt H5 tus xs tvs _ _ H7).
-    destruct H6 as [? [? ?]].
-    forward; inv_all; subst. 
-    rewrite typ_cast_typ_refl. 
-    pose proof exprD'_lift RSym_sym tus nil (rev xs) tvs e t0.
-    simpl in H11. rewrite rev_length in H11. rewrite app_nil_r in H8.
-    forward.
-    eexists. split; [reflexivity|].
-    intros. simpl. inv_all; subst; rewrite Heq. 
-    inv_all; subst. 
-    unfold valid_env in Henv.
-    specialize (Henv _ H7 us vs).
-    apply valid_arg_none_inv in Henv.
-    destruct Henv.
-    specialize (H10 us vs).
-    transitivity (((pt_quant pt (ILFun_Ops (typD ts nil t0)) (fun vs' : hlist (typD ts nil) (rev xs) => t5 us (hlist_app vs' vs)))) (t3 us vs)).
-    Focus 2.
-    destruct H10.
-    split. apply H15. apply H10.
-    destruct vars; simpl in *.
-    admit.
-    split.
-    specialize (H13 us HList.Hnil).
-    destruct pt; simpl in *.
-    adm
-    admit.
-    destruct pt; simpl in *.
-    apply lforallR. intro. apply lforallL with x0.
-    specialize (H11 (fun v => t6 us (hlist_app v vs))).
-    etransitivity; [|eapply H11].
-    etransitivity.
-    destruct vars. simpl in *.
-    Check @existT.
-    assert ( (fun x : hlist (typD ts nil) (rev xs) => t5 us (hlist_app x vs)) = f0) by admit.
-    change (fun x : hlist (typD ts nil) (rev xs) => t5 us (hlist_app x vs)) with f0.
-    setoid_rewrite H11 at 1.
-    inversion H16.
-    eapply f_equal in H16.
-    specialize (H10 (t3 us vs)). .
-    Print existT.
-    inversion H16.
-    Check existT.
-    setoid_rewrite <- H6.
-    einversion Henv. 
-    setoid_rewrite <- H10.
-    destruct Henv as [? [_ Henv]].
-    specialize (Henv us vs). inversion Henv. subst.
-    inv_all; subst.
-    specialize (H13 us HList.Hnil).
-    rewrite UIP_refl in Heq.
-    forward.
-    pose proof(@add_quants_typeof_expr tus tvs _ _ _ (fold_right tyArr t (x::l)) _ H5 ).
-    assert (typeof_expr tus tvs (add_quants pt (tyArr x (fold_right tyArr t l)) xs f) = Some (tyArr x (fold_right tyArr t l))).
-    
-    rewrite add_quants_typeof_expr in H6. forward.
-    Lemma exprD'_lift_arg
-    	(H : exprD' tus (xs ++ ys ++ zs) (App f (lift (length xs) (length ys) e)) t = Some de
-    	exrpD' tus (xs ++ ys ++ zs) (App f
-    
-    apply exprD'_add_quants_app_Some in H2. 
-    apply (apps_rewrite (e2 := App (add_quants pt (tyArr x (fold_right tyArr t l)) xs f) e)) in H1.
-    apply apps_rewrite in H1.
-    apply IHrs.    
-    admit.
-    admit. apply H3.
-    destruct vars. simpl.
-    
-    
-
-         destruct H5; split; [apply H5 | apply H6].
-         Local Transparent ILFun_Ops.
-         apply H5.
-         unfold lentails in H5. simpl in H5.
-         Transparent ILFun_Ops.
-         simpl in *.
-         assert (t3 us vs |-- de2 us vs).
-         apply f_equal.
-         exists t3.
-         specialize
-       	 inv_all; subst.
-       	       	    simpl.
-       	    unfold PQR_aux, TD, Teval.
-       	    forward; inv_all; subst.
-       	    forward.
-       	    
-       	    
-Lemma test : 
-       	    unfold PQR_aux, TD, Teval.
-       	    forward. inv_all; subst.
- 			simpl in *.
-       	    specialize (IHrs _ Hf).
-       	+ simpl.
-       	  inversion Hrs; simpl in *; revert Hf Heq. revert ft. subst; simpl; intros; destruct modes.
-       	  * eapply PQR_atom; try assumption.
-       	  * destruct o.
-       	    - destruct p. eapply PQR_atom; assumption.
-       	    - eapply PQR_atom; assumption.
-       + destruct a; simpl in *; inversion Hrs; revert Heq Hf; revert ft; subst; simpl; intros; clear Hrs.
-         destruct modes.
-         * unfold PQR_aux, TD, Teval. simpl.
-         
-         
-         eapply IHrs; try eassumption.   
-           destruct H2; simpl in *. forward; inv_all; subst. forward.
-           replace (length xs) with (length (rev xs)) by admit.
-           replace (rev xs ++ tvs) with (nil ++ rev xs ++ tvs) by reflexivity.
-           rewrite typeof_expr_lift. simpl. forward.
-           intros.
-           Print PQR_aux.
-           apply Heq.
-      	   pose proof (@exprD'_pull_empty tus tvs).     
-		   intros.
-		   red_exprD; forward; inv_all; subst.
-		   specialize (Heq df).
-		   apply Heq.           
-       	  * inversion Hrs; simpl in *; revert ILOpsf Hft Heq. revert ft. subst; simpl; intros.
-       	    eapply PQR_atom; try assumption. 
-       	  * destruct o. destruct p. eapply PQR_atom; eassumption. eapply PQR_atom; eassumption.
-       	+ simpl. 
-       	  destruct modes.
-       	  * destruct a. simpl. inversion Hrs; subst.
-       	    eapply IHrs. apply H3. simpl in *. apply Htg.
-       	    intros. red_exprD. forward. inv_all; subst.
-       	    apply Heq.
-			destruct H2.
-			
-       	    apply ve_nil. intros. reflexivity.
-       	  * destruct o.
-       	    - destruct p, a; simpl in *. forward.
-       	      inversion Hrs; subst. clear Hrs. simpl in *. destruct H3.
-       	      specialize (H1 v p).
-       	      
-     Lemma PQR_var t pt tus tvs e f g (ILOps : ILogicOps (typD ts nil t)) (_ : (gs t = Some ILOps))
-        (Hf : exists df, exprD' tus tvs f t = Some df)
-     	(Hef : forall de df, exprD' tus tvs e t = Some de -> exprD' tus tvs f t = Some df -> forall us vs, de us vs |-- df us vs) 
-     	(HPQR : PQR_aux CoVariant pt t g e tus tvs) :
-     	PQR_aux CoVariant pt t g f tus tvs.
-     Proof.
-       destruct Hf.
-       unfold PQR_aux, TD, Teval in *. forward; inv_all; subst.
-       rewrite HPQR, Hef; reflexivity. 
-     Qed.
-       
-     destruct vars.
-     eapply PQR_var.
-     admit.
-     SearchAbout typeof_expr exprD'.
-     clear IHrs. clear H4 H1 Henv H H0.
-     generalize dependent (map fst rs). generalize dependent tvs. generalize dependent f; generalize dependent e; induction xs; intros. 
-     destruct pt. simpl.
-     apply typeof_expr_exprD'_impl. assumption.
-     apply typeof_expr_exprD'_impl. assumption.
-     simpl in *.
-     
-     
-
-     replace (S (length xs)) with (length xs + 1) in Ht by omega.
-     rewrite <- app_assoc in Ht; simpl.       
-     rewrite <- lift_lift' in Ht.
-     rewrite <- lift_lift in Ht.
-     rewrite lift_apps in Ht.
-     
-       
-     rewrite lift_app in Ht. simpl in Ht.
-     destruct (IHxs _ _ _ _ Ht); clear IHxs.
-     destruct pt.
-     exists (fun us vs => Forall x, x0 us (HList.Hcons x vs)).
-	 rewrite <- lift_lift'.
-	 replace (S (length xs)) with (length xs + 1) by omega.
-	 rewrite <- lift_lift, lift_apps, lift_app.
-	 simpl. red_exprD; forward; inv_all; subst.
-     assert (gs t = Some ILOps) by admit.
-     forward; inv_all; subst.
-     red_exprD. forward. rewrite typ_cast_typ_refl.
-     inv_all; subst. reflexivity.
-     admit. 
-     Focus 2.
-     rewrite lift_lift. 
-     replace (length l + length xs) with (length xs + length l) by omega.
-     rewrite lift_lift_1. simpl.
-     rewrite <- lift_app.
-     apply IHrs.
-     inv_all; subst.
-     forward.
-     Check exprD'_lift.
-     remember ( exprD' tus (a :: tvs)
-      (add_forall xs t
-         (lift' 0 (S (length xs)) (apps (App f e) (map fst rs)))) t).
-     destruct o.
-	 admit.
-     red_exprD.
-     exists (fun us vs => Forall x, x0 us (HList.Hcons x vs)).
-     red_exprD; forward; inv_all; subst.
-     assert (gs t = Some (ILOps)) by admit.
-     forward. inv_all; subst.
-     red_exprD. forward. rewrite typ_cast_typ_refl.
-     inv_all; subst. reflexivity.
-     admit. intros.
-     Focus 2. 
-     
-     
-     specialize (IHrs (l ++ xs) _ H4).
-     apply IHrs. 
-     rewrite rev_app_distr. rewrite <- app_assoc.
-     assert (App f (lift (length l) (length xs) e0) = lift (length l) (length xs) (App f e0)).
-     destruct (length xs). simpl. reflexivity.
-     simpl. 
-     rewrite typeof_expr_lift.
-     SearchAbout List.rev List.app.
-     f_equal. 
-     Require Import FunctionalExtensionality.
-     apply functional_extensionality.
-     intros.
-     apply functional_extensionality; intros.
-     reflexivity.
-     simpl in *.
-     Focus 3.
-     eapply IHrs.
-     eapply H4.
-     Focus 2.
-     inversion Henv; subst.
-     eapply H7.
-     eapply H7.
-     rewrite <- app_assoc.
-     SearchAbout lift typeof_expr.
-     SearchAbout typeof_expr apps.
-     SearchAbout typeof_expr apps.
-     SearchAbout type_of_applys.
-     SearchAbout apps lift.
-     admit.
-     Focus 2.
-     intros.
-     erewrite type_of_applys_typeof.
-     simpl.
-     Print type_of_applys.
-     SearchAbout type_of_applys.
-     Focus 2.
-     rewrite typeof_expr_lift.
-     rewrite typeof_expr_lift.
-     SearchAbout lift typeof_expr.
-     SearchAbout List.rev List.app.
-     rewrite rev_app_distr. rewrite <- app_assoc.
-     Focus 2.intros.
-     induction xs. simpl.
-     unfold add_quant. destruct pt. simpl. forward.
-     SearchAbout exprD' apps.
-     rewrite exprD'_apps.
-     Focus 23 	      
-     Lemma PQR_covar t pt tus tvs e f g de df (ILOps : ILogicOps (typD ts nil t)) (_ : (gs t = Some ILOps))
-     	(He : exprD' tus tvs e t = Some de)
-     	(Hf : exprD' tus tvs f t = Some df) 
-     	(Hef : forall us vs, de us vs |-- df us vs) 
-     	(HPQR : He : exprD' tus tvs e t = Some de -> exprD' tus tvs f t = Some df PQR_aux ContraVariant pt t g f tus tvs) :
-     	PQR_aux ContraVariant pt t g e tus tvs.
-     Proof.
-       unfold PQR_aux, TD, Teval in *. forward; inv_all; subst.
-       rewrite <- HPQR, Hef; reflexivity. 
-     Qed.
-
-     Lemma add_quant pt xs t (apps (App f e) args)
-       	      
-       	    - destruct a. apply IHrs. apply Ht.
-       	      inversion Henv. subst. apply H0.
-     Qed.
-     Lemma PQR_atomic vars pt t xs f tus tvs : PQR_aux vars pt t (xs, f) (add_quant pt xs t f) tus tvs.
-     Proof.
-       unfold PQR_aux, TD, Teval.
-       forward. destruct vars; intros; reflexivity.
-     Qed.
-     
-     induction rs. simpl.
-     apply PQR_app_nil. simpl.
-     assert (exists ILOps, (gs t) = Some ILOps) by admit. destruct H2.
-     assert (exists f, l = Inj f) by admit. destruct H3 as [f H3]. subst.
-     destruct a. simpl.
-     unfold pq_app.
-     
-     
-     Lemma Happ_aux
-     
-     unfold PQR; intros. simpl.
-     unfold TD. simpl.
-     simpl.
-     unfold pq_app. simpl. destruct a.
-     unfold PQR; intros. simpl. unfold TD. simpl. unfold Teval. simpl.
-     unfold PQR, TD, Teval.
-     forward; inv_all; subst.
-     assert (valid_env tus tvs (Inj f) (pq_env f pt vars)) by admit.
-     
-     Lemma Happ_aux tus tvs pt vars l f rs t e de modes xs (ILOps : ILogicOps (typD ts nil t)) (IL : ILogic (typD ts nil t))
-        (H : exprD' tus tvs
-    	     match pt with
-       		 | PAll => add_forall l t e
-        	 | PExists => add_exists l t e
-       	     end t = Some de) 
-       	(Htyp : typeof_expr tus tvs (apps f (map fst rs)) = Some t)
-       	(Henv : valid_env tus tvs f modes)
-       	(Happ : pq_app_aux tus tvs modes (xs, f) rs = (l, e)) : 
-       	     match pt with
-       	     | PAll => match exprD' tus tvs (add_forall xs t (apps f (map fst rs))) t with
-				| Some q =>
-				    match vars with
-				    | CoVariant =>
-				        forall (us : HList.hlist (typD ts nil) tus)
-				          (vs : HList.hlist (typD ts nil) tvs), de us vs |-- q us vs
-				    | ContraVariant =>
-				        forall (us : HList.hlist (typD ts nil) tus)
-				          (vs : HList.hlist (typD ts nil) tvs), q us vs |-- de us vs
-				    end
-				| None => False
-				end
-		    | PExists => match exprD' tus tvs (add_exists xs t (apps f (map fst rs))) t with
-				| Some q =>
-				    match vars with
-				    | CoVariant =>
-				        forall (us : HList.hlist (typD ts nil) tus)
-				          (vs : HList.hlist (typD ts nil) tvs), de us vs |-- q us vs
-				    | ContraVariant =>
-				        forall (us : HList.hlist (typD ts nil) tus)
-				          (vs : HList.hlist (typD ts nil) tvs), q us vs |-- de us vs
-				    end
-				| None => False
-				end
-		    end.
-     Proof.
-       generalize dependent f; generalize dependent l; generalize dependent modes; generalize dependent pt; generalize dependent vars. generalize dependent xs.
-       induction rs; intros.
-       + simpl in *.
-         destruct modes.
-         * simpl in *. inv_all. subst.
-           destruct pt, vars; forward; inv_all; subst; reflexivity.
-         * simpl in *. destruct o. destruct p; inv_all; subst;
-           destruct pt, vars; forward; inv_all; subst; reflexivity.
-           inv_all; subst. destruct pt, vars; forward; inv_all; subst; reflexivity.
-       + simpl.
-         destruct a. simpl in *.
-         destruct modes; simpl in *.
-         * inv_all; subst; simpl in *. 
-           specialize (IHrs xs vars pt).
-           eapply IHrs.
-           apply H. apply Htyp.
-           apply ve_nil; intros; reflexivity.
-           apply Happ.
-         * destruct o. 
-           - destruct p.
-             inversion Henv; subst.
-             eapply IHrs.
-             eapply H.
-             apply Htyp.
-             apply H4.
+            eapply blarf.
+            eassumption.
+            clear H28.
              
-             apply Happ.
-             inversion Henv. subst.
-             simpl in *.
-           - eapply IHrs.
-             apply H. apply Htyp.
-             Focus 2. apply Happ.
-             inversion Henv. subst. apply H1.
-   Qed.
-             eapply ve_none; intros. reflexivity.
-         destruct p. simpl in *.
-           destruct pt, vars; forward; inv_all; subst.
-           eapply IHrs.
-         eapply IHrs.
-         apply H.
-         apply Htyp.
-         admit.
-         destruct modes.
-         simpl in *.
-         apply Happ.
-         destruct modes.
-         simpl.
-           inversion Henv. forward.
-    Qed.
-    
-    eapply Happ_aux.
-    eassumption.
-    eassumption.
-    eassumption.
-     *)
-     (*
-     induction rs.
-     + simpl in *.
-       destruct (pq_env f pt vars). simpl in *. inv_all; subst.
-       destruct vars, pt; simpl in *; forward; inv_all; subst; reflexivity.
-       simpl in *. destruct o. destruct p. inv_all; subst.
-       destruct vars, pt; simpl in *; forward; inv_all; subst; reflexivity.
-       inv_all; subst.
-       destruct vars, pt; simpl in *; forward; inv_all; subst; reflexivity.
-     + simpl.
-       apply IHrs.
-       destruct (pq_env f CoVariant 
-     generalize dependent ts0. generalize dependent t. generalize dependent l.
-     induction rs; simpl in *.
-     + intros; apply PQR_app_nil.
-     + simpl in *; intros.
-       simpl.
-       destruct l.
-       admit.
-       admit.
-       admit.
-       rewrite typeof_expr_apps in H; [congruence|]. 
-       simpl. forward.
-       admit.
-       
-       SearchAbout typeof_expr App.
-        
-        
-        forward. simpl.
-       SearchAbout typeof_expr
-       unfold type_of_apply. destruct t0; try reflexivity.
-       simpl in *.
-       cases (typ_eqb t0_1 t1).
-       case (typ_eqb t0_1 t1).
-       destruct a. simpl. forward.
-       inversion H1; subst. clear H1.
-       destruct a; simpl in *.
-       destruct H6.
-       specialize (IHrs _ _ H _ H2).
-	   unfold pq_app. simpl.
-       SearchAbout typeof_expr apps.
-       Check type_of_applys_typeof.
-       
-       Lemma type_of_applys_typeofE  : forall (ts : types) (sym : Type) (RSym_sym : RSym (typD ts) sym)
-      									      (tus tvs : tenv typ) (es : list (expr sym)) (e : expr sym) (t : typ),
-          typeof_expr tus tvs e = Some t ->
-          typeof_expr tus tvs (apps e es) = type_of_applys RSym_sym tus tvs t es
-       
-       erewrite type_of_applys_typeof in H.
-       Focus 2.
-       SearchAbout typeof_expr apps.
-       
-       Lemma typeof_expr_apps_App tus tvs f e rs t (H : typeof_expr tus tvs (apps (App f e) rs) = Some t) :
-       	 exists te, typeof_expr tus tvs f = Some (tyArr te t) /\ typeof_expr tus tvs (apps e rs) = Some te.
-       Proof.
-         generalize dependent e.
-         induction rs.
-         + simpl in *. forward. unfold type_of_apply in H1. forward. inv_all; subst.
-           exists t1. intuition.
-         + simpl in *. intros.
-           apply IHrs. simpl in *.
-           exists (tyArr t1 t3), t1.
-       Lemma PQR_typeof_expr pt vars t l f tus tvs IL (H : PQR pt vars t l f tus tvs) 
-                             (HIL : gs t = Some IL) :
-                             typeof_expr tus tvs l = Some t.
-       Proof.
-         unfold PQR, TD, Teval in H. forward.
-         destruct vars, pt. inv_all; subst.
-       
-       
-       simpl. forward.  
-       inv_all; subst. forward.     
-       simpl in H1.
-       destruct H0.
-       simpl in H1.
-       unfold PQR, TD, Teval.
-       simpl.
-       rewrite exprD'_apps.
-       forward.
-       inv_all; subst.
-       destruct a. simpl.
-       SearchAbout apps_sem.
-       simpl in *.
-       
-       red_exprD.
-       unfold PQR, TD, Teval in IHrs.
-       forward.
-       Print apps_sem'.
-       Check apps_sem.
-       Print ExprD3.EXPR_DENOTE_core.exprD'.
-       Print apps_sem.
-       Print apply_sem.
-       Check exprD_apps.
-Qed.
-
-       Lemma exprD'_apps : forall (ts : types) (sym : Type) (RSym_sym : RSym (typD ts) sym)
-         (us vs : env (typD ts)) (es : list (expr sym)) (e : expr sym)
-         (t : typ),
-       exprD' (typeof_env us) (typeof_env vs) (apps e es) t = apps_sem RSym_sym us vs e es t.
-       
-       destruct a. simpl in *.
-       unfold PQR, TD, Teval.
-       Check
-       forward. inv_all; subst.
-       simpl in *.
-       destruct pt, vars. forward. simpl in *.
-       Print apps.
-       
-Check exprD_apps.
-
-Check apps_sem.
-       
-       rewrite exprD_apps.
-       SearchAbout apps.
-       SearchAbout typeof_expr apps.
-       erewrite type_of_applys_typeof in H.
-       Focus 2. simpl. forward. forward. inv_all; subst. forward.
-       simpl in H.
-       unfold PQR, TD, Teval in *; simpl in *.
-       simpl.
-       inversion H2; subst; intros.
-       simpl in *; clear H2. destruct H6.
-       unfold PQR, TD, Teval. simpl.
-       forward. inv_all; subst.
-       SearchAbout typeof_expr.
-       destruct vars. forward.
-       destruct l. 
-       red_exprD. simpl in H. forward. red_exprD.
-       SearchAbout ExprDI.nth_error_get_hlist_nth.
-       replace ft with t.
-       apply ft.
-       destruct l. 
-       admit.
-       red_exprD; forward; simpl in *.
-       uip_all'.
-       forward.
-       admit.
-       forward.
-       forward.
-       destruct pt, vars.
-       red_exprD. simpl.
-       simpl in *.
-       admit.
-       admit.
-       forward.
-       destruct vars, pt.
-       rewrite ft in .
-       forward; inv_all; subst.
-       rewrite pqapp_nil in H3.
-       inv_all; subst.
-       destruct vars. 
-       destruct pt. forward.
-       red_exprD.
-       progress forward.
-       progress forward.
-       forward; inv_all; subst.
-       destruct vars; simpl in *.
-       destruct vars. simpl in *.
-       destruct pt, vars; simpl in *.
-       inversion H1.
-       apply Forall2_refl in H1.
-       apply Forall2_ind.
-       SearchAbout Forall2.
-       forward; inv_all; subst.
-       destruct pt, vars. simpl.
-       forward.
-       unfold pq_app in H3. destruct l.
-       simpl in *. inv_all; subst. forward.
-       forward. destruct vars.
-       destruct vars. simpl in *.
-       destruct pt. forward.
-     
-   Qed.
-
-  Lemma add_quants_app tus tvs xs ys t p q d (IL : ILogicOps (typD ts nil t))
-  	(H : exprD' tus tvs (add_quants (xs ++ ys) t (App (lift 0 (length ys) p) (lift (length ys) (length xs) q))) t = Some d) :
-    exists tq dp dq,
-      typeof_expr (typeof_env tus) (rev ys ++ tvs) q = Some tq /\
-      exprD' tus tvs (add_quants xs (tyArr tq t) p) (tyArr tq t) = Some dp /\ exprD' tus tvs (add_quants ys tq q) tq = Some dq /\
-      forall vs, d vs |-- (dp vs) (dq vs).
-  Proof.
-
-
-  Lemma exprD'_add_quants_cons_Some (Ty : typ) (IL_Ty : ILogicOps (typD ts nil Ty))
-        (_ : gs Ty = Some IL_Ty)
-  : forall tus tvs tm a b x,
-      exprD' tus tvs (add_quants (a :: b) Ty tm) Ty = Some x ->
-      exists y,
-        exprD' tus (a :: tvs) (add_quants b Ty tm) Ty = Some y /\
-        forall g, x g -|- lexists (fun v => y (HList.Hcons v g)).
-  Proof.
-    simpl.
-    intros.
-    red_exprD. forward. subst.
-    revert H4. inv_all. subst Ty. subst i.
-    intros. inv_all. subst p.
-    revert H5. subst.
-    red_exprD. forward. subst.
-    inv_all. subst.
-    eexists. split.
-    { reflexivity. }
-    { intros.
-      unfold typeof_sym in *. simpl in *.
-      rewrite H in *.
-      red_exprD. uip_all.
-      inv_all. subst.
-      reflexivity. }
-  Qed.
-
-  Require Import ExtLib.Data.HList.
-
-  Lemma exists_hlist_app (Ty : typ) (ILO_Ty : ILogicOps (typD ts nil Ty))
-        (IL_Ty : ILogic (typD ts nil Ty))
-  : forall xs ys (P : _ -> typD ts nil Ty),
-      Exists v : HList.hlist (typD ts nil) (xs ++ ys), P v -|-
-                                                         Exists v : HList.hlist (typD ts nil) xs,
-    Exists v' : HList.hlist (typD ts nil) ys, P (HList.hlist_app v v').
-  Proof.
-    split.
-    { apply lexistsL; intros.
-      rewrite <- hlist_app_hlist_split with (h := x).
-      eapply lexistsR.
-      eapply lexistsR.
-      reflexivity. }
-    { do 2 (apply lexistsL; intros).
-      eapply lexistsR.
-      reflexivity. }
-  Qed.
-
-  Lemma lexists_iff_2 (Ty : Type) (ILO_Ty : ILogicOps Ty)
-        (IL_Ty : ILogic Ty)
-  : forall T U (P Q : T -> U -> Ty),
-      (forall a b, P a b -|- Q a b) ->
-      Exists x : T, Exists y : U, P x y -|-
-                                    Exists y : U, Exists x : T, Q x y.
-  Proof.
-    split.
-    { apply lexistsL; intros.
-      apply lexistsL; intros.
-      eapply lexistsR; eauto.
-      eapply lexistsR; eauto. eapply H. }
-    { apply lexistsL; intros.
-      apply lexistsL; intros.
-      eapply lexistsR; eauto.
-      eapply lexistsR; eauto. eapply H. }
-  Qed.
-
-(* Why both lemmas? *)
-
-  Lemma lexists_iff_2_rw (Ty : Type) (ILO_Ty : ILogicOps Ty)
-        (IL_Ty : ILogic Ty)
-  : forall T U (P Q : T -> U -> Ty),
-      (forall a b, P a b -|- Q a b) ->
-      Exists x : T, Exists y : U, P x y -|-
-                                    Exists y : U, Exists x : T, Q x y.
-  Proof.
-    apply lexists_iff_2. apply _.
-  Qed.
-
-  Lemma exprD'_add_quants_rev_Some (Ty : typ) (ILO_Ty : ILogicOps (typD ts nil Ty))
-        (_ : gs Ty = Some ILO_Ty) :
-    forall tus xs tvs tm dtm,
-      exprD' tus (rev xs ++ tvs) tm Ty = Some dtm ->
-      exists dtm',
-        exprD' tus tvs (add_quants xs Ty tm) Ty = Some dtm' /\
-        forall vs, dtm' vs -|- lexists (fun vs' => dtm (HList.hlist_app vs' vs)).
-  Proof.
-    induction xs; simpl; intros.
-    + exists dtm. split; [assumption|].
-      intros. split.
-      * apply lexistsR with Hnil. simpl. reflexivity.
-      * apply lexistsL; intros. rewrite (hlist_eta x). simpl. reflexivity.
-    + specialize (IHxs (a::tvs) tm).
-      assert ((rev xs ++ a :: nil) ++ tvs = rev xs ++ a :: tvs).
-      { rewrite app_ass. reflexivity. }
-      rewrite exprD'_var_env with (H := H1) in IHxs.
-      rewrite H0 in IHxs.
-      specialize (IHxs (fun x => match H1 in _ = vs return hlist (typD ts nil) vs -> typD ts nil Ty with
-                                   | eq_refl => dtm
-                                 end x)).
-      destruct IHxs.
-      { clear.
-        generalize dependent ((rev xs ++ a :: nil) ++ tvs).
-        intros; subst. (** eta **) reflexivity. }
-      { destruct H2.
-        red_exprD.
-        rewrite H.
-        red_exprD.
-        rewrite H.
-        red_exprD.
-        rewrite H2. eexists; split; eauto.
-        simpl.
-        intros.
-        split.
-        { apply lexistsL; intros.
-          specialize (H3 (Hcons x0 vs)).
-          rewrite H3.
-          apply lexistsL; intros.
-          eapply (lexistsR (hlist_app x1 (Hcons x0 Hnil))).
-          change (Hcons x0 vs) with (hlist_app (Hcons x0 Hnil) vs).
-          rewrite hlist_app_assoc; eauto with typeclass_instances.
-          match goal with
-            | |- _ ?X |-- _ match _ with eq_refl => ?Y end =>
-              change Y with X; generalize X
-          end.
-          generalize (app_ass_trans (rev xs) (a :: nil) tvs).
-          generalize H1. simpl. rewrite <- H1.
-          uip_all. reflexivity. }
-        { apply lexistsL; intros.
-          rewrite <- (hlist_app_hlist_split _ _ x0).
-          apply (lexistsR (hlist_hd (snd (hlist_split (rev xs) (a :: nil) x0)))).
-          rewrite H3.
-          apply (lexistsR (fst (hlist_split (rev xs) (a :: nil) x0))).
-          rewrite hlist_app_assoc; eauto with typeclass_instances.
-          rewrite (hlist_eta (snd (hlist_split (rev xs) (a :: nil) x0))).
-          simpl.
-          rewrite (hlist_eta (hlist_tl (snd (hlist_split (rev xs) (a :: nil) x0)))).
-          simpl. intros.
-          match goal with
-            | |- _ match _ with eq_refl => ?X end |-- _ ?Y =>
-              change Y with X; generalize X
-          end.
-          generalize (app_ass_trans (rev xs) (a :: nil) tvs).
-          generalize H1. simpl. rewrite <- H1.
-          uip_all. reflexivity. } }
-  Qed.
-
-  Lemma exprD'_add_quants_app_Some (Ty : typ) (ILO_Ty : ILogicOps (typD ts nil Ty))
-        (_ : gs Ty = Some ILO_Ty)
-  : forall tus a tvs tm b x,
-      exprD' tus tvs (add_quants (a ++ b) Ty tm) Ty = Some x ->
-      exists y,
-        exprD' tus (rev a ++ tvs) (add_quants b Ty tm) Ty = Some y /\
-        forall g, x g -|- lexists (fun v => y (HList.hlist_app v g)).
-  Proof.
-    induction a.
-    { simpl.
-      intros. eexists; split; eauto.
-      intros.
-      split.
-      { eapply lexistsR. instantiate (1 := Hnil). reflexivity. }
-      { apply lexistsL. intros. rewrite (hlist_eta x0). reflexivity. } }
-    { simpl List.app.
-      intros.
-      eapply exprD'_add_quants_cons_Some in H0; eauto.
-      destruct H0 as [ ? [ ? ? ] ].
-      eapply IHa in H0.
-      destruct H0 as [ ? [ ? ? ] ].
-      generalize dependent x1.
-      assert ((rev a0 ++ a :: nil) ++ tvs = rev a0 ++ a :: tvs).
-      { rewrite app_ass. reflexivity. }
-      intros.
-      exists (fun z =>
-                x1 match H0 in _ = t return HList.hlist (typD ts nil) t with
-                     | eq_refl => z
-                   end).
-      generalize H.
-      change (a :: tvs) with ((a :: nil) ++ tvs) in *.
-      assert (forall g : HList.hlist (typD ts nil) tvs,
-                x g -|- Exists v : HList.hlist (typD ts nil) (a :: nil), x0 (HList.hlist_app v g)).
-      { intros. specialize (H1 g).
-        rewrite H1.
-        split.
-        { apply lexistsL; intros.
-          eapply lexistsR; intros.
-          instantiate (1 := Hcons x2 Hnil). reflexivity. }
-        { apply lexistsL; intros.
-          eapply lexistsR. instantiate (1 :=  hlist_hd x2).
-          rewrite (hlist_eta x2).
-          rewrite (hlist_eta (hlist_tl x2)). reflexivity. } }
-      clear H1.
-      simpl rev.
-      generalize dependent (a :: nil).
-      intros.
-      split.
-      { generalize H0. rewrite H0. uip_all.
-        reflexivity. (** eta **) }
-      { intros.
-        rewrite H4.
-        rewrite exists_hlist_app; eauto with typeclass_instances.
-        setoid_rewrite H3.
-        eapply lexists_iff_2; eauto with typeclass_instances.
-        intros.
-        rewrite HList.hlist_app_assoc; eauto with typeclass_instances.
-        uip_all. reflexivity. } }
-  Qed.
-
-  Lemma exprD'_add_quants_all_Some (Ty : typ) (ILO_Ty : ILogicOps (typD ts nil Ty))
-        (_ : gs Ty = Some ILO_Ty)
-  : forall tus a tvs tm x,
-      exprD' tus tvs (add_quants a Ty tm) Ty = Some x ->
-      exists y,
-        exprD' tus (rev a ++ tvs) tm Ty = Some y /\
-        forall g, x g -|- lexists (fun v => y (HList.hlist_app v g)).
-  Proof.
-    intros.
-    rewrite <- (app_nil_r a) in H0.
-    apply exprD'_add_quants_app_Some in H0; eauto.
-  Qed.
-
-  Local Existing Instance EqDec_typ.
-
-  Lemma hlist_app_nil A F (xs : list A) (hnil : hlist F nil) (hys : hlist F xs) : hlist_app hnil hys = hys.
-  Proof.
-    assert (hnil = Hnil) by apply hlist_nil_eta.
-    rewrite H. reflexivity.
-  Qed.
-  Lemma hlist_app_nil A F (xs : list A) (hnil : hlist F nil) (hys : hlist F xs) : hlist_app hnil hys = hys.
-  Proof.
-    assert (hnil = Hnil) by apply hlist_nil_eta.
-    rewrite H. reflexivity.
-  Qed.
-
-  Lemma hlist_app_cons A F (xs ys : list A) (x : A) (el : F x) (hxs : hlist F xs) (hys : hlist F ys) :
-    Hcons el (hlist_app hxs hys) = hlist_app (Hcons el hxs) hys.
-  Proof.
-    simpl. reflexivity.
-  Qed.
-
-  Lemma lift_entails tus xs ys zs e t de df (HILops : ILogicOps (typD ts nil t)) (HIL: ILogic (typD ts nil t))
-	(He : exprD' tus (xs ++ ys ++ zs) (lift (length xs) (length ys) e) t = Some de)
-	(Hf : exprD' tus (xs ++ zs) e t = Some df)
-	(hxs : hlist (typD ts nil) xs)
-	(hys : hlist (typD ts nil) ys)
-	(hzs : hlist (typD ts nil) zs) :
-    de (hlist_app hxs (hlist_app hys hzs)) |-- df (hlist_app hxs hzs).
-  Proof.
-    induction ys; intros; simpl in *.
-    + rewrite hlist_app_nil.
-      rewrite He in Hf. inversion Hf. reflexivity.
-    + replace (S (length ys)) with (1 + length ys) in He by omega.
-      rewrite <- lift_lift', <- lift_lift in He.
-      pose proof (exprD'_lift RSym_sym tus xs (a::nil) (ys++zs) (lift (length xs) (length ys) e) t).
-      simpl in *. forward; inv_all; subst.
-      specialize (IHys t1).
-      specialize (H1 hxs (Hcons (hlist_hd hys) Hnil) (hlist_app (hlist_tl hys) hzs)).
-      simpl in H1.
-      rewrite hlist_app_cons, <- hlist_cons_eta in H1.
-      rewrite H1 at 1. apply IHys. reflexivity.
-  Qed.
-
-  Lemma add_quants_app tus tvs xs ys t p q d (IL : ILogicOps (typD ts nil t))
-  	(H : exprD' tus tvs (add_quants (xs ++ ys) t (App (lift 0 (length ys) p) (lift (length ys) (length xs) q))) t = Some d) :
-    exists tq dp dq,
-      typeof_expr (typeof_env tus) (rev ys ++ tvs) q = Some tq /\
-      exprD' tus tvs (add_quants xs (tyArr tq t) p) (tyArr tq t) = Some dp /\ exprD' tus tvs (add_quants ys tq q) tq = Some dq /\
-      forall vs, d vs |-- (dp vs) (dq vs).
-  Proof.
-    eapply exprD'_add_quants_app_Some in H; eauto.
-    destruct H as [ ? [ ? ? ] ].
-    rewrite <- (app_nil_r ys) in H.
-    eapply exprD'_add_quants_app_Some in H; eauto.
-    destruct H as [ ? [ ? ? ] ].
-    simpl in H.
-    red_exprD; forward; inv_all; subst.
-    rewrite app_nil_r in *.
-    pose proof (exprD'_lift RSym_sym tus (rev ys) (rev xs) tvs q t1).
-    repeat rewrite rev_length in H. forward; inv_all; subst. simpl.
-    pose proof (exprD'_lift RSym_sym tus nil (rev ys) (rev xs ++ tvs) p (tyArr t1 t)).
-    repeat rewrite rev_length in H4. simpl in H4. forward; inv_all; subst.
-    assert (ILogicOps (typD ts nil (tyArr t1 t))) by admit.
-    apply exprD'_add_quants_rev_Some in H7.
-    destruct H7 as [? [? ?]].
-    assert (ILogicOps (typD ts nil t1)) by admit.
-    apply exprD'_add_quants_rev_Some in H5.
-    destruct H5 as [? [? ?]].
-    exists t1, x0, x1.
-    split. admit.
-    split. assumption. split. assumption.
-    intros.
-    assert (ILogic (typD ts nil t)) by admit.
-    rewrite H0. apply lexistsL; intros.
-    rewrite H1. apply lexistsL; intros.
-    assert (t3 (hlist_app x3 (hlist_app x2 vs)) |-- x0 vs).
-    assert (ILogic (typD ts nil t1 -> typD ts nil t)) by admit.
-    rewrite H7. apply lexistsR with x2.
-    specialize (H8 Hnil x3 (hlist_app x2 vs)).
-    simpl in H8. rewrite H8. reflexivity.
-    assert (t4 (hlist_app x3 (hlist_app x2 vs)) |-- x1 vs).
-    assert (ILogic (typD ts nil t1)) by admit.
-    rewrite H9. apply lexistsR with x3.
-    specialize (H6 x3 x2 vs). rewrite H6. reflexivity.
-
-  Lemma hlist_app_cons A F (xs ys : list A) (x : A) (el : F x) (hxs : hlist F xs) (hys : hlist F ys) :
-    Hcons el (hlist_app hxs hys) = hlist_app (Hcons el hxs) hys.
-  Proof.
-    simpl. reflexivity.
-  Qed.
-  Abort.
-  (* This lemma is true with a bit more help, the problem comes from the requirement to have ILogics for partially applied functions, which is more or less trivial,
- 		   but an extra Proper requirement is also needed that allows us to prove (f p |-- g q) if (f |-- g) and (p |-- q). The problem here is also that these propers need
- 		   to be preserved when the existential quantifiers are stripped. This is true, but requires lemmas such as exprD'_add_quants_app_Some to keep track of that information
- 		   as well. The question is if we want a lemma that is as general as this one, or if we are happy with the special cases. *)
-
-  Lemma lift_entails tus xs ys zs e t de df (HILops : ILogicOps (typD ts nil t)) (HIL: ILogic (typD ts nil t))
-	(He : exprD' tus (xs ++ ys ++ zs) (lift (length xs) (length ys) e) t = Some de)
-	(Hf : exprD' tus (xs ++ zs) e t = Some df)
-	(hxs : hlist (typD ts nil) xs)
-	(hys : hlist (typD ts nil) ys)
-	(hzs : hlist (typD ts nil) zs) :
-    de (hlist_app hxs (hlist_app hys hzs)) |-- df (hlist_app hxs hzs).
-  Proof.
-    induction ys; intros; simpl in *.
-    + rewrite hlist_app_nil.
-      rewrite He in Hf. inversion Hf. reflexivity.
-    + replace (S (length ys)) with (1 + length ys) in He by omega.
-      rewrite <- lift_lift', <- lift_lift in He.
-      pose proof (exprD'_lift RSym_sym tus xs (a::nil) (ys++zs) (lift (length xs) (length ys) e) t).
-      simpl in *. forward; inv_all; subst.
-      specialize (IHys t1).
-      specialize (H1 hxs (Hcons (hlist_hd hys) Hnil) (hlist_app (hlist_tl hys) hzs)).
-      simpl in H1.
-      rewrite hlist_app_cons, <- hlist_cons_eta in H1.
-      rewrite H1 at 1. apply IHys. reflexivity.
-  Qed.
-
-  Lemma Happ
-  : forall tus tvs l (l_res : T) rs t ts,
-      typeof_expr (typeof_env tus) tvs (apps l (map fst rs)) = Some t ->
-      let ft := fold_right tyArr t ts in
-      PQR ft l (l_res (typeof_env tus) tvs) tus tvs ->
-      Forall2 (fun t x =>
-                    typeof_expr (typeof_env tus) tvs (fst x) = Some t
-                 /\ PQR t (fst x) (snd x (typeof_env tus) tvs) tus tvs)
-              ts rs ->
-      PQR t (apps l (map fst rs)) (pq_app l l_res rs (typeof_env tus) tvs) tus tvs.
-   Proof.
-     intros; unfold PQR, TD, Teval in *.
-     destruct l; simpl in *; try apply I.
-     destruct i; simpl in *; try apply I.
-     * red_exprD; forward; inv_all; subst; simpl in *.
-       red_exprD; forward; inv_all; subst.
-       rewrite H0 in H5. inversion H5; subst.
-       reflexivity.
-     * forward; inv_all; subst. simpl in *.
-       forward; inv_all; subst; simpl in *.
-       red_exprD; forward; inv_all; subst; simpl in *.
-       forward; inv_all; subst.
-       red_exprD; forward; inv_all; subst.
-       red_exprD; forward; inv_all; subst.
-       red_exprD; forward; inv_all; subst.
-       inversion H9; clear H9; simpl in *.
-       revert H0. revert ft. subst. intros.
-       inversion H10; clear H10; simpl in *.
-       revert H0. revert ft. subst. intros. simpl in *.
-       inversion H12; clear H12; revert H0; revert ft; subst; intros.
-       simpl in *.
-       destruct H8, H9.
-       forward; inv_all; subst.
-       rewrite H1 in H7; rewrite H2 in H4; inv_all;
-       revert H0; revert ft; subst; intros.
-       forward; inv_all; revert H0; revert ft; subst; intros.
-       forward; inv_all; subst.
-       red_exprD; forward; inv_all; subst.
-       red_exprD; forward; inv_all; subst.
-       red_exprD; forward; inv_all; subst.
-	   red_exprD; forward; inv_all; subst.
-
-
-       eapply exprD'_add_quants_app_Some in H3; eauto.
-       destruct H3 as [ ? [ ? ? ] ].
-       rewrite <- (app_nil_r l3) in H3.
-       eapply exprD'_add_quants_app_Some in H3; eauto.
-       destruct H3 as [ ? [ ? ? ] ].
-       simpl in H3.
-       red_exprD.
-       rewrite H in *.
-       forward. subst.
-       rewrite app_nil_r in *.
-       inv_all. subst.
-       red_exprD.
-       forward. inv_all. subst i. subst t.
-       subst p. subst t5. rewrite x1 in H21.
-       inv_all. clear H8. clear H6.
-       red_exprD.
-       simpl in H13. rewrite H in *.
-       forward. inv_all. subst t. subst t9.
-       inv_all. subst p.
-       inversion x2. subst t8. revert H5. subst t4.
-       inv_all. subst t0.
-       repeat match goal with
-                | H : ?X = ?X |- _ => clear H
-              end.
-       simpl in H16. forward.
-       subst t7. revert H6. revert x2. clear H5.
-       intro. rewrite (UIP_refl x2).
-       clear x2.
-       clear H0.
- 		pose proof (exprD'_lift RSym_sym tus (rev l3) (rev l2) tvs e4 x0).
- 		repeat rewrite rev_length in H0. forward; inv_all; subst. simpl.
- 		pose proof (exprD'_lift RSym_sym tus nil (rev l3) (rev l2 ++ tvs) e3 x0).
- 		repeat rewrite rev_length in H8. simpl in H8. forward; inv_all; subst.
-        apply exprD'_add_quants_rev_Some in H12; eauto; destruct H12 as [? [? ?]].
-        apply exprD'_add_quants_rev_Some in H3; eauto; destruct H3 as [? [? ?]].
-        forward; inv_all; subst.
-        assert (ILogic (typD ts nil x0)) by admit.
-        rewrite H4. apply lexistsL; intros.
-        rewrite H6. apply lexistsL; intros.
-        apply landR.
-        + apply landL1.
-          rewrite <- H20. rewrite H15.
-          apply lexistsR with x3.
-          specialize (H13 Hnil x4 (hlist_app x3 vs)). simpl in H13. rewrite H13. reflexivity.
-        + apply landL2.
-          rewrite <- H18. rewrite H16. apply lexistsR with x4.
-          rewrite H5. reflexivity.
-    * forward; inv_all; subst. simpl in *.
-       forward; inv_all; subst; simpl in *.
-       red_exprD; forward; inv_all; subst; simpl in *.
-       forward; inv_all; subst.
-       red_exprD; forward; inv_all; subst.
-       red_exprD; forward; inv_all; subst.
-       red_exprD; forward; inv_all; subst.
-       inversion H9; clear H9; simpl in *.
-       revert H0. revert ft. subst. intros.
-       inversion H10; clear H10; simpl in *.
-       revert H0. revert ft. subst. intros. simpl in *.
-       inversion H12; clear H12; revert H0; revert ft; subst; intros.
-       simpl in *.
-       destruct H8, H9.
-       forward; inv_all; subst.
-       rewrite H1 in H7; rewrite H2 in H4; inv_all;
-       revert H0; revert ft; subst; intros.
-       forward; inv_all; revert H0; revert ft; subst; intros.
-       forward; inv_all; subst.
-       red_exprD; forward; inv_all; subst.
-       red_exprD; forward; inv_all; subst.
-       red_exprD; forward; inv_all; subst.
-	   red_exprD; forward; inv_all; subst.
-
-
-       eapply exprD'_add_quants_app_Some in H3; eauto.
-       destruct H3 as [ ? [ ? ? ] ].
-       rewrite <- (app_nil_r l3) in H3.
-       eapply exprD'_add_quants_app_Some in H3; eauto.
-       destruct H3 as [ ? [ ? ? ] ].
-       simpl in H3.
-       red_exprD.
-       rewrite H in *.
-       forward. subst.
-       rewrite app_nil_r in *.
-       inv_all. subst.
-       red_exprD.
-       forward. inv_all. subst i. subst t.
-       subst p. subst t5. rewrite x1 in H21.
-       inv_all. clear H8. clear H6.
-       red_exprD.
-       simpl in H13. rewrite H in *.
-       forward. inv_all. subst t. subst t9.
-       inv_all. subst p.
-       inversion x2. subst t8. revert H5. subst t4.
-       inv_all. subst t0.
-       repeat match goal with
-                | H : ?X = ?X |- _ => clear H
-              end.
-       simpl in H16. forward.
-       subst t7. revert H6. revert x2. clear H5.
-       intro. rewrite (UIP_refl x2).
-       clear x2.
-       clear H0.
- 		pose proof (exprD'_lift RSym_sym tus (rev l3) (rev l2) tvs e4 x0).
- 		repeat rewrite rev_length in H0. forward; inv_all; subst. simpl.
- 		pose proof (exprD'_lift RSym_sym tus nil (rev l3) (rev l2 ++ tvs) e3 x0).
- 		repeat rewrite rev_length in H8. simpl in H8. forward; inv_all; subst.
-        apply exprD'_add_quants_rev_Some in H12; eauto; destruct H12 as [? [? ?]].
-        apply exprD'_add_quants_rev_Some in H3; eauto; destruct H3 as [? [? ?]].
-        forward; inv_all; subst.
-        assert (ILogic (typD ts nil x0)) by admit.
-        rewrite H4. apply lexistsL; intros.
-        rewrite H6. apply lexistsL; intros.
-        apply lorL.
-        + apply lorR1.
-          rewrite <- H20. rewrite H15.
-          apply lexistsR with x3.
-          specialize (H13 Hnil x4 (hlist_app x3 vs)). simpl in H13. rewrite H13. reflexivity.
-        + apply lorR2.
-          rewrite <- H18. rewrite H16. apply lexistsR with x4.
-          rewrite H5. reflexivity.
-   Qed.
-
-End PullQuant.
-
-Section TestPullQuant.
-
-  Context {A : Type} {ILO : ILogicOps A}.
-
-  Context (logics_sound : forall g, match logics g with
-                                  | Some T => @ILogic _ T
-                                  | None => unit
-                                end).
-
-  Variable eq_nat : nat -> nat -> A.
-  Definition ts : types := (default_type A)::(default_type nat)::nil.
-  Variable es : embed_ops ts.
-  Variable funcs : fun_map ts.
-  Definition logics : logic_ops ts :=
-    fun t => match t with
-               | tyType 0 => Some ILO
-               | tyProp => Some _
-               | _ => None
-             end.
-
-  Definition test_fold := fun x => TD (es := es) (funcs) logics (tyType 0) (app_fold_args pqArgs x nil nil).
-
-  Eval cbv - [land ltrue lexists] in test_fold inj_true nil nil.
-  Eval cbv - [land ltrue lexists] in test_fold (inj_and inj_true inj_true) nil nil.
-  Eval cbv - [land ltrue lexists] in test_fold
-                   (inj_and (inj_exists (tyType 1) (inj_and inj_true (inj_exists (tyType 1) inj_true))) inj_true) nil nil.
-  Eval cbv - [land ltrue lexists] in test_fold
-                   (inj_and (inj_exists (tyType 0) (Var 0)) (inj_exists (tyType 0) (Var 0))) nil nil.
- Eval cbv - [land ltrue lexists] in test_fold
-                   (inj_exists (tyType 1)
-                                        (inj_exists (tyType 0) (Var 0))) nil nil.
-  Eval compute in test_fold
-                   (inj_and (inj_exists (tyType 1) (inj_and inj_true
-                                                            (inj_exists (tyType 2) (Var 0))))
-                            inj_true) nil nil.
-Print inj_exists.
-Definition test_fold := @setoid_fold _ _ _ (atomic (SRW_Algo_pull_quant logics)) (SetoidFold.app (SRW_Algo_pull_quant logics))
-                   (SetoidFold.abs (SRW_Algo_pull_quant logics)) nil nil.
-
-Eval compute in test_fold (Abs (tyType 1) inj_true) (Rpointwise (tyType 1) (Rinj ent)).
-Eval compute in test_fold (Inj (ilf_exists (tyType 1) (tyType 0))) (Rfunctorial (Rpointwise (tyType 1) (Rinj ent)) (Rinj ent)).
-
-
-
-Eval compute in
-  Eval compute in
-      @setoid_fold _ _ _ (atomic SRW_Algo_pull_quant) (SetoidFold.app SRW_Algo_pull_quant)
-                   (SetoidFold.abs SRW_Algo_pull_quant) nil nil
-                   (inj_and (inj_exists (tyType 1) (inj_eq_nat (Var 0) (Var 0))) inj_true)
-                   (Rinj ent).
-  simpl.
-Check @setoid_fold.
-  Eval compute in
-      @setoid_fold _ _ _ _ _ properAt atomic app nil (Inj And) (tyProp :: nil)
-                      (PRfunctorial (PRguess _ tyProp) (PRfunctorial (PRguess _ tyProp) (PRinj Impl))).
-
-End TestPullQuant.
-
-    Variable TT : Type.
-    Let T := tenv typ -> tenv typ -> TT.
-
-    Variable do_var : var -> T.
-    Variable do_uvar : uvar -> T.
-    Variable do_inj : sym -> T.
-    Variable do_abs : typ -> expr sym -> T -> T.
-    Variable do_app : expr sym -> T ->
-                      list (expr sym * T) -> T.
-
-    Definition semArgs : AppFullFoldArgs TT :=
-      @Build_AppFullFoldArgs TT do_var do_uvar do_inj do_abs do_app.
-
-    Variable R : forall t, typD ts nil t -> TT -> env (typD ts) -> env (typD ts) -> Prop.
-    Hypothesis Hvar : forall us tvs t v val,
-                        exprD' us tvs (Var v) t = Some val ->
-                        forall vs,
-                          R t (val vs) (do_var v (typeof_env us) tvs) us (join_env vs).
-    Hypothesis Huvar : forall us tvs t v val,
-                        exprD' us tvs (UVar v) t = Some val ->
-                        forall vs,
-                          R t (val vs) (do_uvar v (typeof_env us) tvs) us (join_env vs).
-    Hypothesis Hinj : forall us tvs t v val,
-                        exprD' us tvs (Inj v) t = Some val ->
-                        forall vs,
-                          R t (val vs) (do_inj v (typeof_env us) tvs) us (join_env vs).
-    (** INTERESTING ONES **)
-    Hypothesis Habs : forall us tvs t t' e e_res val,
-                        exprD' us (t :: tvs) e t' = Some val ->
-                        forall (vs : hlist (typD ts nil) tvs),
-                          (forall x,
-                             R t' (val (Hcons x vs)) (e_res (typeof_env us) (t :: tvs))
-                               us ((@existT _ (typD ts nil) t x) :: join_env vs)) ->
-                          R (tyArr t t') (fun x => val (Hcons x vs))
-                            (do_abs t e e_res (typeof_env us) tvs) us (join_env vs).
-
-
-Section Relation.
-	Variable ts : types.
-	Variable func : Type.
-	Variable R : RSym (typD ts) func.
-	Variable us vs : tenv typ.
-
-	Definition is_relation_bool (t : typ) :=
-		match t with
-			| tyArr t (tyArr t' tyProp) => t ?[eq] t'
-			| _                          => false
-		end.
-
-	Definition is_relation (e : expr func) (t : typ) :=
-		WellTyped_expr us vs e (tyArr t (tyArr t tyProp)).
-
-End Relation.
-
-Section IsPreOrder.
-	Variable ts : types.
-	Variable func : Type.
-	Variable us vs : env (typD ts).
-	Variable R : RSym (typD ts) func.
-
-	Variable is_preorder : expr func -> bool.
-
-	Definition preorder_prop (e : expr func) (t : typ) :=
-		forall v, exprD us vs e (tyArr t (tyArr t tyProp)) = Some v ->
-		PreOrder v.
-
-	Definition is_preorder_sound :=
-	    forall e, is_preorder e = true -> forall t, preorder_prop e t.
-
-End IsPreOrder.
-
-Section PullExistsLeft.
-  Context (ts : types) (funcs : fun_map ts) (gs : logic_ops ts).
-
-  Local Instance RSym_sym : SymI.RSym (typD ts) ilfunc := RSym_ilfunc ts funcs gs.
-
-  Variable us vs : env (typD ts).
-  Definition T := (list typ * list typ * expr ilfunc)%type.
-
-  Definition T_union (p q : T) : T :=
-    match p, q with
-        (a1, b1, c1), (a2, b2, c2) =>
-        (a1 ++ a2, b1 ++ b2, App (lift 0 ((length a2) + (length b2)) c1) c2)
-    end.
-
-  Fixpoint T_to_expr_aux (vs qs : list typ) e t :=
-    match vs, t with
-      | nil, _ => Some (fold_right (fun v e => App (Inj (ilf_exists v t)) (Abs v e))
-                                   e qs)
-      | v::vs, tyArr a t =>
-        match T_to_expr_aux vs qs e t, v ?[eq] a with
-          | Some x, true => Some (Abs a x)
-          | _, _ => None
-        end
-      | _, _ => None
-    end.
-
-  Definition T_to_expr (e : T) (t : typ) :=
-    match e with
-        (vs, qs, e) => T_to_expr_aux vs qs e t
-    end.
-
-  Inductive Rbase :=
-    | Ent t : (exists v, gs' ts gs t = Some v) -> Rbase
-    | Eq : Rbase.
-
-  Fixpoint Rbase_eq (r1 r2 : Rbase) : bool :=
-    match r1, r2 with
-      | Ent t1 _, Ent t2 _ => t1 ?[eq] t2
-      | Eq, Eq             => true
-      | _, _               => false
-    end.
-
-  Instance RelDec_Rbase_eq : RelDec (@eq Rbase) := { rel_dec := Rbase_eq }.
-
-  Definition typeForRbase r :=
-    match r with
-      | Ent t _ => t
-      | Eq => tyProp
-    end.
-
-  Definition app (vs us : tenv typ) (pq p : T) (rpq rp : R Rbase) : option T :=
-    match rpq with
-      | Rinj (Ent t _) => Some (T_union pq p)
-      | Rpointwise a (Rinj (Ent t _)) =>
-        match pq, p with
-          | ((tyArr a' t')::nil, a''::nil, Var 1), (a'''::ls, es, p) =>
-            if a' ?[eq] a'' && a'' ?[eq] a''' then
-              Some (ls, a''::es, p)
-            else
-              None
-          | _, _ => None
-        end
-      | _ => None
-    end.
-
-  Definition abs (vs us : tenv typ) (t : typ) (p : T) (r : R Rbase) : option T :=
-    Some (t :: fst (fst p), snd (fst p), snd p).
-
-  Fixpoint unify (r : R Rbase) (p : PR Rbase) : bool :=
-    match p with
-      | PRguess => true
-      | PRinj i => match r with
-                     | Rinj i' => i ?[ eq ] i'
-                     | _ => false
-                   end
-      | PRfunctorial a b =>
-        match r with
-          | Rfunctorial a' b' => andb (unify a' a) (unify b' b)
-          | _ => false
-        end
-      | PRpointwise t a =>
-        match r with
-          | Rpointwise t' a' => andb (t ?[eq] t') (unify a' a)
-          | _ => false
-        end
-    end.
-
-  Definition proper_lookup (a : expr ilfunc)  (r : Rbase) : option (R Rbase) :=
-    match a, r with
-      | Inj (ilf_and t), Ent t' pr =>
-        if t ?[eq] t' then
-          Some (Rfunctorial (Rinj (Ent pr)) ((Rfunctorial (Rinj (Ent pr)) (Rinj (Ent pr)))))
-        else
-          None
-      | Inj (ilf_exists a t), Ent t' pr =>
-        if t ?[eq] t' then
-          Some (Rfunctorial (Rpointwise a (Rinj (Ent pr))) (Rinj (Ent pr)))
-        else
-          None
-      | Inj (ilf_true t), Ent t' pr => if t ?[eq] t' then Some (Rinj (Ent pr)) else None
-(*      | _, Ent (tyType 0) pr => match @typeof_expr (@ILogicFunc.ts A) ilfunc (RSym_sym funcs logics) nil nil a with
-                               | Some (tyType 0) => Some (Rinj (Ent pr))
-                               | _ => None
-                                end*)
-      | _, _ => None
-    end.
-
-
-
-  Fixpoint get_proper_aux (e : expr ilfunc) (r : PR Rbase) : option (R Rbase) :=
-    match r with
-      | PRinj r => proper_lookup e r
-      | PRfunctorial l r => get_proper_aux e r
-      | PRpointwise t r => get_proper_aux e r
-      | _ => None
-    end.
-
-  Definition get_unified_proper (e : expr ilfunc) (r : PR Rbase) : option (R Rbase) :=
-    match get_proper_aux e r with
-      | Some x => if unify x r then Some x else None
-      | None => None
-    end.
-
-  Lemma unification_instantiates r r' (H : unify r' r = true) :
-    instantiates r' r.
-  Proof.
-
-    generalize dependent r; induction r'; simpl; intros.
-    + destruct r0; try congruence; [|apply Ins_guess]. admit.
-    + destruct r; try congruence; [apply Ins_guess|].
-      rewrite andb_true_iff in H. apply Ins_func; [apply IHr'1| apply IHr'2]; intuition.
-    + destruct r; try congruence; [apply Ins_guess|].
-      rewrite andb_true_iff in H.
-      assert (t = t0) by admit; subst.
-      apply Ins_point. apply IHr'; intuition.
-  Qed.
-
-  Definition atom (us vs : tenv typ) (e : expr ilfunc) (r : R Rbase) : option T :=
-    match e with
-      | Inj (ilf_exists a t) => Some ((tyArr a t)::nil, a::nil, Var 1)
-      | _ => Some (nil, nil, e)
-    end.
-
-  Lemma atom_cases (tus tvs : tenv typ) (e : expr ilfunc) (r : R Rbase) (res : T)
-    (H : atom tus tvs e r = Some res) :
-    (exists a t, (e = Inj (ilf_exists a t) /\ (res =  ((tyArr a t)::nil, a::nil, Var 1)))) \/
-    (res = (nil, nil, e)).
-  Proof.
-    destruct e; simpl in *; try (right; congruence).
-    destruct i; simpl in *; try (right; congruence).
-    left. exists t; exists t0. intuition congruence.
-  Qed.
-
-  Definition TD us vs (e : T) (t : typ) :=
-    match (T_to_expr e t) with
-      | Some x => exprD' us vs x t
-      | None   => None
-    end.
-
-
-  Require Import FunctionalExtensionality.
-
-  Lemma TD_abs uvs vvs avs a b c t x
-    (H : TD uvs vvs (a::avs, b, c) t = Some x) :
-      exists x, t = tyArr a x.
-  Proof.
-    unfold TD in H.
-    destruct t; simpl in *; try congruence.
-    forward; inv_all; subst. exists t2. reflexivity.
-  Qed.
-
-  Lemma TD_abs_list uvs vvs avs b c t x
-    (H : TD uvs vvs (avs, b, c) t = Some x) :
-      exists y, t = fold_right tyArr y avs.
-  Proof.
-    generalize dependent t; generalize dependent vvs.
-    induction avs; intros; simpl in *.
-    + exists t; reflexivity.
-    + unfold TD, T_to_expr in H; simpl.
-      red_exprD; forward; inv_all; subst.
-      unfold TD, T_to_expr in IHavs.
-      red_exprD; forward; inv_all; subst.
-      specialize (IHavs _ _ t). rewrite H0 in IHavs.
-      destruct (IHavs H1) as [y Hy].
-      exists y. rewrite Hy. reflexivity.
-  Qed.
-
-  Lemma TD_abs_sem uvs vvs avs a b c t x :
-    TD uvs vvs (a::avs, b, c) (tyArr a t) = Some x <->
-    TD uvs (a::vvs) (avs, b, c) t = Some (fun g => x (HList.hlist_tl g) (HList.hlist_hd g)).
-  Proof.
-    split; intro H.
-    + unfold TD, T_to_expr in H; simpl in H.
-      red_exprD; forward; inv_all; subst.
-      red_exprD; forward; inv_all; subst.
-      rewrite x0.
-      unfold TD, T_to_expr. rewrite H. rewrite H2.
-      f_equal. apply functional_extensionality; intros x.
-      rewrite <- HList.hlist_cons_eta. reflexivity.
-    + unfold TD, T_to_expr in *; simpl in *.
-      forward. red_exprD; forward. inv_all; subst.
-      rewrite typ_cast_typ_refl.
-      f_equal.
-  Qed.
-
-  Fixpoint typD_fold_right tvs uvs t avs :
-    typD tvs uvs (fold_right tyArr t avs) -> HList.hlist (typD tvs uvs) avs ->
-    typD tvs uvs t :=
-    match avs with
-      | nil => fun x _ => x
-      | a::avs => fun f lst => typD_fold_right (f (HList.hlist_hd lst)) (HList.hlist_tl lst)
-    end.
-(*
-  Lemma TD_abs_list_sem uvs vvs avs b c t x :
-    (TD uvs vvs (avs, b, c) (fold_right tyArr t avs) = Some x) <->
-    TD uvs ((rev avs) ++ vvs) (nil, b, c) t =
-    Some (fun g => match HList.hlist_split (rev avs) vvs g with
-                     | (a, b) => typD_fold_right (x b) a
-                   end).
-  Proof.
-    split; intro H.
-    + generalize dependent t; generalize dependent vvs.
-      induction avs; simpl in *; intros.
-      * rewrite H. f_equal.
-      * apply TD_abs_sem in H.
-        apply IHavs in H.
-        admit.
-    + generalize dependent t; generalize dependent vvs.
-      induction avs; simpl in *; intros.
-      * rewrite H. reflexivity.
-      * admit.
-  Qed.
-*)
-
-  Lemma TD_quant_sem_aux uvs vvs e t a (v : typD ts nil a) x :
-    TD uvs (a::vvs) e t = Some x <->
-    TD uvs vvs e t = Some (fun vs => x (HList.Hcons v vs)).
-  Proof.
-    split; intro H.
-    + unfold TD in *; simpl in *; forward.
-      pose proof (exprD'_lower RSym_sym us nil (a::nil) vvs e0).
-      simpl in *.
-
-      red_exprD.
-      forward.
-      pose proof (exprD'_lift RSym_sym us nil (a::nil) vvs e0 t).
-
-      simpl in *.
-      SearchAbout lift.
-    simpl.
-
-
-
-
-  Lemma TD_quant_sem_aux uvs vvs q qs c t x IL (a : typD ts nil q)
-        (HIL : gs' ts gs t = Some IL)
-        (H : TD uvs vvs (nil, q::qs, c) t = Some x) :
-        exists f, x = (fun vs => lexists (f vs)) /\
-                    TD uvs vvs (nil, qs, c) t = Some (fun vs => f vs a).
-  Proof.
-    unfold TD, T_to_expr in *; simpl in H.
-    red_exprD; forward; inv_all; revert H4; generalize dependent t2; subst; intros.
-    destruct x0. subst.
-    red_exprD; forward; inv_all; subst.
-    simpl in *. forward; inv_all; subst.
-    exists (fun x a => t (HList.Hcons a x)).
-    split. simpl.
-    apply functional_extensionality; intros x1; simpl.
-    uip_all. reflexivity.
-    rewrite H2.
-    destruct x0.
-rewrite <- H7 in H5.
-rewrite <- H7 in x0. rewrite H7 in H5.
-    red_exprD; forward; inv_all; uip_all.
-    rewrite HIL in *. rewrite <- H6 in *. rewrite H7 in *. rewrite x0 in *.
-    red_exprD; forward; inv_all. simpl in *. forward. inv_all.
-    red_exprD; forward; inv_all; revert H4; generalize dependent t2; subst; intros.
-    rewrite typ_cast_typ_refl in H2.
-    simpl.
-    red_exprD; forward; inv_all.
-    f_equal. generalize dependent t2; subst; intros.
-    apply functional_extensionality; intros; simpl.
-    red_exprD; forward; inv_all; subst; simpl in *.
-    f_equal. apply functional_extensionality. intros; simpl.
-    admit.
-  Qed.
-
-  Lemma TD_quant_sem uvs vvs q qs c il t f IL
-        (HIL : gs' ts gs t = Some IL)
-        (H : TD uvs (q::vvs) (nil, qs, c) il t = Some f) :
-    TD uvs vvs (nil, qs, c) il t = Some (fun g => lexists (fun x => f (HList.Hcons x g))).
-  Proof.
-    unfold TD, T_to_expr in *.
-    simpl in *. remember ((fold_right
-           (fun (t : typ) (e : expr ilfunc) =>
-            App (Inj (ilf_exists t il)) (Abs t e)) c qs)) as y.
-    admit.
-  Qed.
-
-
-
-  Fixpoint RD (r : R Rbase) : (typD ts nil (typeForR typeForRbase r)) ->
-                              (typD ts nil (typeForR typeForRbase r)) -> Prop :=
-    match r with
-      | Rfunctorial l r => fun f g => forall x y, @RD l x y -> @RD r (f x) (g y)
-      | Rinj (Ent t _) =>
-        fun a b => t ?[eq] typeForR typeForRbase r = true /\
-                   exists ILO, gs' ts gs t = Some ILO /\ a |-- b
-      | Rinj Eq => fun a b => a = b
-      | Rpointwise t r => fun f g => forall x, @RD r (f x) (g x)
-    end.
-
-  Lemma RD_reflexive r a : @RD r a a.
-  Proof.
-    induction r.
-    + simpl. destruct r; [|reflexivity].
-      split. simpl. apply rel_dec_eq_true. apply _. reflexivity.
-      destruct e. simpl in *.
-      exists x. intuition. admit.
-    + simpl; intros.
-      admit. (* This is not true *)
-    + simpl; intros.
-      apply IHr.
-  Qed.
-
-  Definition TR us vs (r : R Rbase) (t : T) v : Prop :=
-    match TD us vs t (typeForR typeForRbase r) with
-      | Some x => forall vs, @RD r v (x vs)
-      | None => False
-    end.
-
-  Theorem Happ
-  : forall us vs t1 t2 r1 r2 v1 v2 f result,
-      app (typeof_env us) (typeof_env vs) r1 r2 t1 t2 = Some result ->
-      exprD us vs f (typeForR typeForRbase (Rfunctorial t1 t2)) = Some v1 ->
-      @TR us (typeof_env vs) (Rfunctorial t1 t2) r1 v1 ->
-      @TR us (typeof_env vs) t1 r2 v2 ->
-      @TR us (typeof_env vs) t2 result (v1 v2).
-  Proof.
-    intros. simpl in *.
-    destruct r1 as [[rv1 re1] r1], r2 as [[rv2 re2] r2]; simpl in *.
-    unfold TR in *.
-    forward. simpl in *.
-Check TD.
-    (f : typD ts nil r ->
-     (H: TD us0 (typeof_env vs0) (r::rv1, re1, r1)
-         (tyArr ) =
-       Some t0)
-       TD us0 (typeof_env vs0) (rv1, re1, r1)
-         (tyArr (typeForR typeForRbase t1) (typeForR typeForRbase t2)) =
-       Some f
-
-    unfold TD in H1.
-
-
-
-    destruct t1; simpl in *; try congruence.
-    destruct r; simpl in *; try congruence.
-    inv_all; subst. unfold T_union; simpl.
-    unfold TR, TD, T_to_expr. simpl.
-    forward.
-    induction rv1. simpl. admit.
-    simpl in *.
-Eval compute in (typD ts nil (typeForR typeForRbase (Rpointwise a t2))).
-    Lemma TR_abs t uvs vvs r a rvs es p (v : typD ts nil (typeForR typeForRbase t))
-      (H : forall (x : typD ts nil a), exists f rd, f x = v /\ rd = Rpointwise a r /\ @TR uvs vvs (Rpointwise a r) (rvs, es, p) f) :
-      @TR uvs vvs r (a :: rvs, es, p) v.
-    Proof.
-      admit.
-    Qed.
-
-    apply TR_abs.
-    intros.
-
-    apply TR_abs. apply IHrv1.
-
-    inv_all; subst. unfold T_union; simpl.
-    unfold TR in *.
-    remember (TD us0 (typeof_env vs0) r1
-           (typeForR typeForRbase (Rfunctorial t1 t2))) as o.
-    destruct o; simpl in *; [|intuition].
-    remember (TD us0 (typeof_env vs0) r2 (typeForR typeForRbase t1)) as o.
-    destruct o; simpl in *; [|intuition].
-    destruct t1; simpl in *; try congruence.
-    destruct r; simpl in *; try congruence.
-    induction rv1. simpl. admit.
-    unfold TD, T_to_expr; simpl.
-    SearchAbout exprD' Abs.
-    red_exprD.
-    destruct t2; simpl in *; try congruence.
-    destruct r; simpl in *; try congruence.
-    destruct t2; simpl in *; try congruence.
-    unfold TD in IHrv1. simpl in *.
-    apply IHrv1.
-    remember (TD us0 (typeof_env vs0)
-       (a :: rv1 ++ rv2, re1 ++ re2,
-       App (lift 0 (length rv2 + length re2) r1) r2)
-       (typeForR typeForRbase t2)) as o.
-    destruct o; intros; simpl in *.
-    unfold TD, T_to_expr in Heqo.
-    simpl in Heqo.
-    red_exprD. forward.
-    unfold TR.
-    unfold TD.
-    unfold T_to_expr.
-    simpl.
-    unfold TR, TD, T_to_expr in H1; simpl in *.
-    unfold exprD in H1.
-    destruct vs0.
-    remember (exprD' us0 tvs
-            (Abs a
-               (fold_right Abs
-                  (fold_right
-                     (fun (t0 : typ) (e : expr ilfunc) =>
-                      App
-                        (Inj
-                           (ilf_exists t0
-                              (tyArr t (typeForR typeForRbase t2))))
-                        (Abs t0 e)) r1 re1) rv1))
-            (tyArr t (typeForR typeForRbase t2))).
-SearchAbout expr
-    red_exprD.
-    simpl in H1.
-    red_exprD.
-    simpl.
-    simpl.
-
-    simpl.
-    simpl.
-
-destruct H1RD as [_ H1RD].
-    unfold app in H.
-    unfold TD, T_to_expr in *; simpl in *.
-    destruct t1; simpl in *; try congruence.
-    destruct r; simpl in *; try congruence.
-    unfold TD in H1.
-    unfold app in H; simpl in *.
-    simpl in *.
-
-
-    Lemma TD_app us vs e1 e2 t1 t2 tr1 tr2 result
-          (H1 : TD us vs e1 (tyArr t1 t2) = Some tr1)
-          (H2 : TD us vs e2 t1 = Some tr2)
-          (H3 : app (typeof_env us) (typeof_env vs) r1 r2 t1 t2 = Some result) :
-      TD us vs result t2 = Some (tr1 tr2).
-
-
-    unfold TD in *.
-
-    specialize (H1RD _ _ H2RD). simpl in *.
-    simpl in *.
-    unfold TR.
-    exists (v1 v2).
-    split; [|admit].
-    clear H1
-    red_exprD.
-    unfold TR.
-    unfold TD in *.
-    unfold T_to_expr in *.
-    simpl in *.
-  Theorem Hatomic
-    : forall tus tvs e r r' result,
-        get_unified_proper  e r = Some r' ->
-        (atom tus tvs e r' = Some result) ->
-        @setoid_fold_spec _ _ (RSym_sym) _ _ _ TR tus tvs e r result r'.
-  Proof.
-    intros; repeat split; intros.
-    + apply unification_instantiates.
-      unfold get_unified_proper in H.
-      destruct (get_proper_aux e r); try congruence.
-      remember (unify r0 r) as b; destruct b; congruence.
-    + unfold get_unified_proper in H.
-      remember (get_proper_aux e r) as o; destruct o; try congruence.
-      remember (unify r0 r) as b; destruct b; try congruence.
-      inv_all; subst.
-      Print pr_type.
-  Lemma proper_lookup_type tus tvs e r r' r'' t
-        (H : unify r' r = true)
-        (H1 : proper_lookup e r'' = Some r')
-        (H2 : typeof_expr tus tvs e = Some t) :
-      typeForR typeForRbase r' = t.
-  Proof.
-    destruct e; simpl in *; try congruence;
-    destruct i; simpl in *; try congruence;
-    destruct r''; simpl in *; try congruence;
-    destruct e as [v ILV];
-    remember (t0 ?[ eq ] t1) as b;
-    destruct b; try congruence;
-    assert (t0 = t1) by admit; subst;
-    try rewrite ILV in H2; inv_all; subst; simpl; try reflexivity.
-    remember (t1 ?[eq] t2) as b.
-    destruct b; try congruence.
-    inv_all; subst; simpl in *.
-    destruct r; simpl in *; try congruence.
-    assert (t1 = t2) by admit; subst.
-    rewrite ILV in H2; inv_all.
-    assumption.
-    destruct r1; simpl in *; try congruence.
-    assert (t1 = t2) by admit; subst.
-    rewrite ILV in H2; inv_all.
-    destruct r2; simpl in *; try congruence.
-    rewrite andb_true_iff in H; destruct H as [H H1].
-    rewrite andb_true_iff in H; destruct H as [H H0].
-    assert (t1 = t2) by admit; subst.
-    rewrite ILV in H2; inv_all. assumption.
-    admit.
-  Qed.
-
-  Lemma unification_type tus tvs e r r' r'' t (H : unify r' r = true)
-    (H1 : get_proper_aux e r'' = Some r')
-    (H2 : pr_type typeForRbase r t)
-    (H3 : typeof_expr tus tvs e = Some t) : typeForR typeForRbase r' = t.
-  Proof.
-    generalize dependent r; generalize dependent r'; induction r''; simpl; intros;
-    try congruence.
-    eapply proper_lookup_type; eauto.
-    eapply IHr''2; eauto.
-    eapply IHr''; eauto.
-  Qed.
-
-
-  eapply unification_type; eauto.
-    + remember (exprD' us0 tvs e (typeForR typeForRbase r')).
-      destruct o; [|apply I].
-      intros.
-      apply atom_cases in H0; destruct H0 as [[a [t1 [He Hres]]] | H0].
-      subst; unfold TR.
-      unfold TD, T_to_expr; simpl.
-      red_exprD; forward; inv_all; subst; simpl in *.
-      assert (exists IL, gs' ts gs t1 = Some IL) by admit.
-      destruct H4 as [IL H4].
-      rewrite H4 in H0. rewrite H4 in H2. inv_all; simpl in *.
-      subst; red_exprD.
-      remember (typ_cast_typ ts nil (tyArr (tyArr a t1) t1)
-           (typeForR typeForRbase r')) as o.
-      destruct o; try congruence.
-      symmetry in Heqo.
-      apply typ_cast_typ_eq in Heqo; subst.
-      exists t2.
-      split.
-      inv_all; subst.
-      unfold exprD.
-      rewrite split_env_join_env.
-      red_exprD.
-
-      uip_all.
-      rewrite <- Heqo.
-      simpl.
-      uip_all.
-      red_exprD.
-      simpl.
-      red_exprD.
-      eexists.
-
-Check typ_cast_typ_eq.
-rewrite typ_cast_typ_eq in Heqo.
-      SearchAbout typ_cast_typ.
-      red_exprD.
-      assert (t = tyArr (tyArr a t1) t1) by admit.
-      simpl.
-      subst.
-      unfold TR.
-      exists (t0 vs0).
-      split. unfold TD. simpl.
-      unfold exprD; simpl.
-      rewrite split_env_join_env.
-      unfold T_to_expr; simpl.
-      remember (exprD' us0 tvs e (typeForR typeForRbase r')).
-      destruct o; inv_all; subst; [reflexivity|congruence].
-      apply RD_reflexive.
-  Qed.
-
-  Definition SRW_Algo_pull_quant :=
-    @SRW_Algo_properAt ilfunc T Rbase get_unified_proper atom app abs.
-
-End PullExistsLeft.
-
-Section demo.
-  Context {A : Type} {ILO : ILogicOps A}.
-
-  Context (logics_sound : forall g, match logics g with
-                                  | Some T => @ILogic _ T
-                                  | None => unit
-                                end).
-
-  Existing Instance ILFun_ILogic.
-
-  Lemma gs'_sound : forall g, match gs' ts logics g with
-                                | Some T => @ILogic _ T
-                                | None => unit
-                              end.
-  Proof.
-    intros g; induction g; simpl; try apply tt.
-    simpl. remember (gs' ts logics g2) as o; destruct o; [apply _ | apply tt].
-    destruct n; [|apply tt]; simpl in *.
-    specialize (logics_sound (tyType 0)); simpl in *.
-    apply logics_sound.
-  Qed.
-
-  Program Definition ent := @Ent _ logics (tyType 0) _.
-  Next Obligation.
-    exists ILO. reflexivity.
-  Defined.
-
-Print setoid_fold_spec.
-(*
-Check @exprD'.
-Print setoid_fold_spec.
-  Definition TR us vs (r : R (Rbase logics)) (t : T) v : Prop :=
-    exists v', TD us vs t (typeForR typeForRbase r) = Some v' /\ @RD us vs r v v'.
-
-
-  Theorem Hatomic
-    : forall tus tvs e r r' result,
-        (get_unified_proper get_proper)  e r = Some r' ->
-        (atom tus tvs e r' = Some result) ->
-        @setoid_fold_spec _ _ (RSym_sym funcs logics) _ _ _ TR tus tvs e r result r'.
-  Proof.
-    intros.
-    unfold atom in H0. inv_all; subst.
-    red; intros.
-    split. admit.
-    split. admit.
-    intros.
-    remember (exprD' us tvs e (typeForR typeForRbase r')) as o.
-    destruct o; [|apply I].
-    intros.
-    unfold TR. exists (t0 vs).
-    split.
-    unfold TD.
-    unfold exprD.
-    simpl.
-    simpl.
-
-
-
-
-
-  Check SRW_AlgoOk_properAt.
-*)
-  Eval compute in
-      @setoid_fold _ _ _ (atomic (SRW_Algo_pull_quant logics)) (SetoidFold.app (SRW_Algo_pull_quant logics))
-                   (SetoidFold.abs (SRW_Algo_pull_quant logics)) nil nil
-                   inj_true
-                   (Rinj ent).
-
-  Eval compute in
-      @setoid_fold _ _ _ (atomic (SRW_Algo_pull_quant logics)) (SetoidFold.app (SRW_Algo_pull_quant logics))
-                   (SetoidFold.abs (SRW_Algo_pull_quant logics)) nil nil
-                   (inj_and inj_true inj_true)
-                   (Rinj ent).
-
-  Eval compute in
-      @setoid_fold _ _ _ (atomic (SRW_Algo_pull_quant logics)) (SetoidFold.app (SRW_Algo_pull_quant logics))
-                   (SetoidFold.abs (SRW_Algo_pull_quant logics)) nil nil
-                   (inj_and (inj_exists (tyType 1) (inj_and inj_true (inj_exists (tyType 2) inj_true))) inj_true)
-                   (Rinj ent).
-
-Definition test_fold := @setoid_fold _ _ _ (atomic (SRW_Algo_pull_quant logics)) (SetoidFold.app (SRW_Algo_pull_quant logics))
-                   (SetoidFold.abs (SRW_Algo_pull_quant logics)) nil nil.
-
-Eval compute in test_fold (Abs (tyType 1) inj_true) (Rpointwise (tyType 1) (Rinj ent)).
-Eval compute in test_fold (Inj (ilf_exists (tyType 1) (tyType 0))) (Rfunctorial (Rpointwise (tyType 1) (Rinj ent)) (Rinj ent)).
-
-
-
-Eval compute in
-  Eval compute in
-      @setoid_fold _ _ _ (atomic SRW_Algo_pull_quant) (SetoidFold.app SRW_Algo_pull_quant)
-                   (SetoidFold.abs SRW_Algo_pull_quant) nil nil
-                   (inj_and (inj_exists (tyType 1) (inj_eq_nat (Var 0) (Var 0))) inj_true)
-                   (Rinj ent).
-  simpl.
-Check @setoid_fold.
-  Eval compute in
-      @setoid_fold _ _ _ _ _ properAt atomic app nil (Inj And) (tyProp :: nil)
-                      (PRfunctorial (PRguess _ tyProp) (PRfunctorial (PRguess _ tyProp) (PRinj Impl))).
-
-
-Check @SRW_Algo_properAt.
-
-  Check inj_true.
-
-Check @inj_true.
-
-  Axiom eq_nat : nat -> nat -> T.
-
-  Definition eq_nat_emb := F ts (tyArr (tyType 1) (tyArr (tyType 1) (tyType 0))) (eq_nat).
-
-  Definition inj_and (p q : expr ilfunc) : expr ilfunc := App (App (Inj (ilf_and (tyType 0))) p) q.
-
-  Lemma
-
-  Definition inj_true : expr ilfunc := Inj (ilf_true (tyType 0)).
-  Definition inj_false : expr ilfunc := Inj (ilf_false (tyType 0)).
-  Definition inj_exists (a : typ) (f : expr ilfunc) : expr ilfunc :=
-  	App (Inj (ilf_exists a (tyType 0))) (Abs a f).
-  Definition inj_forall (a : typ) (f : expr ilfunc) : expr ilfunc :=
-  	App (Inj (ilf_forall a (tyType 0))) (Abs a f).
-  Definition inj_eq_nat (a b : expr ilfunc) : expr ilfunc :=
-    App (App (Inj (fref (1%positive))) a) b.
-
-
-
-  Definition tm : expr ilfunc := inj_and inj_true inj_true.
-  Definition tm2 : expr ilfunc := inj_forall (tyType 1) (inj_eq_nat (Var 0) (Var 0)).
-  Require Import MirrorCore.Ext.ExprD.
-
-  (** TODO: Here we run into a problem because the [expr] type is
-   ** fixed to the [typ] defined in [MirrorCore.Ext.Types].
-   ** - To solve this problem, we need to abstract [expr] with respect to
-   **   types.
-   **)
-
-  Eval cbv beta iota zeta delta - [ltrue land] in @exprD ts _ (RSym_ilfunc ts funcs logics) nil nil tm (tyType 0).
-  Eval cbv beta iota zeta delta - [ltrue land lforall] in @exprD ts _ (RSym_ilfunc ts funcs logics) nil nil tm2 (tyType 0).
-
-  Check setoid_fold.
-
-End demo.
-
-
-
-  Lemma T_to_expr_app pq p tpq tp vp vpq r
-  	(Hpq : TD pq (tyArr tp tpq) = Some vpq)
-  	(Hp : TD p tp = Some vp) :
-  	TD (app pq p r r) tpq = Some (vpq vp).
-    clear gs_sound.
-    Set Printing All.
-clear gs.
-
-
-
-
-
-  Definition T_to_expr (t : T) (il : typ) : expr ilfunc :=
-    fold_right Abs (fold_right (fun t e => App (Inj (ilf_exists t il))
-                                               (Abs t e)) (snd t) (snd (fst t)))
-               (fst (fst t)).
-
-  Definition T_app (p q : T) : option T :=
-    match p, q with
-      | (l::vp, tp, ep), (nil, tq, eq) =>
-        Some (vp, tp ++ tq, App (lift 0 (length tq)  ep) eq)
-      | _, _ => None
-    end.
-
-
-
-
-
-  Definition Rbase := (typ * expr ilfunc)%type.
-
-  Definition typeForRbase (r : Rbase) : typ := fst r.
-
-  Definition app (p q : T) : T := T_union p q.
-
-
-
-  Definition T := (list typ * list typ * expr ilfunc)%type.
-
-  Definition T_to_expr (t : T) (il : typ) : expr ilfunc :=
-    fold_right Abs (fold_right (fun t e => App (Inj (ilf_exists t il))
-                                               (Abs t e)) (snd t) (snd (fst t)))
-               (fst (fst t)).
-
-  Definition T_app (p q : T) : option T :=
-    match p, q with
-      | (l::vp, tp, ep), (nil, tq, eq) =>
-        Some (vp, tp ++ tq, App (lift 0 (length tq)  ep) eq)
-      | _, _ => None
-    end.
-
-
-
-  Definition T_union (p q : T) : T :=
-  	(fst p ++ fst q, App (lift 0 (length (fst q)) (snd p)) (snd q)).
-
-  Definition Rbase := (typ * expr ilfunc)%type.
-
-  Definition typeForRbase (r : Rbase) : typ := fst r.
-
-  Definition app (p q : T) : T := T_union p q.
-
-
-
-
-   Fixpoint RD (r : R Rbase) : (typD ts nil (typeForR typeForRbase r)) ->
-   (typD ts nil (typeForR typeForRbase r)) -> Prop :=
-  	match r with
-  		| Rfunctorial l r => fun f g => forall x y, @RD l x y -> @RD r (f x) (g y)
-  		| Rinj t => fun a b => exists v, exprD us vs (snd t) (tyArr (fst t) (tyArr (fst t) tyProp)) = Some v /\ v a b
-  		| Rpointwise t r => fun f g => forall x, @RD r (f x) (g x)
-  	end.
-(*
-  Lemma RD_refl (r : R Rbase) a : @RD r a a.
-  Proof.
-  	induction r.
-  	+ simpl.
-  	  Require Import FunctionalExtensionality.
-  	  apply functional_extensionality.
-  	destruct a.
-  	induction a.
-.*)
-  Lemma T_to_expr_app_wt p q tpq tq
-  	(Hp : WellTyped_expr (typeof_env us) (typeof_env vs) (T_to_expr p (tyArr tq tpq)) (tyArr tq tpq))
-  	(Hq : WellTyped_expr (typeof_env us) (typeof_env vs) (T_to_expr q tq) tq) :
-  	WellTyped_expr (typeof_env us) (typeof_env vs) (T_to_expr (app p q) tpq) tpq.
-  Proof.
-  	admit.
-  Qed.
-
-  Lemma T_to_expr_app pq p tpq tp vp vpq
-  	(Hpq : exprD us vs (T_to_expr pq (tyArr tp tpq)) (tyArr tp tpq) = Some vpq)
-  	(Hp : exprD us vs (T_to_expr p tp) tp = Some vp) :
-  	exprD us vs (T_to_expr (app pq p) tpq) tpq = Some (vpq vp).
-  Proof.
-  	unfold T_to_expr in *; simpl in *.
-  	rewrite fold_right_app.
-  	destruct p as [vps p], pq as [vpqs pq]; simpl in *.
-  	induction vps; simpl in *.
-  	SearchAbout exprD lift.
-  	+ generalize dependent vs. clear vs. induction vpqs; simpl in *; intros.
-  	  * rewrite exprD_App.
-  	    assert (typeof_expr (typeof_env us) (typeof_env vs) pq = Some (tyArr tp tpq)) by admit.
-  	    rewrite H0. rewrite Hpq. rewrite Hp.
-  	    rewrite typ_cast_typ_refl. reflexivity.
-  	  * simpl in *.
-  	    red_exprD. forward; subst; inv_all; revert Hpq; subst; intros.
-  	    assert (exists ILTemp, gs tpq = Some ILTemp) by admit.
-  	    destruct H0. rewrite H0.
-  	    red_exprD. forward. inv_all; subst.
-  	    rewrite typ_cast_typ_refl.
-  	    rewrite typ_cast_typ_refl.
-  	    SearchAbout exprD Abs.
-  	    unfold exprD. simpl.
-  	    destruct vs; simpl in *.
-  	    rewrite exprD'_Abs. rewrite typ_cast_typ_refl.
-  	    assert (va : typD ts nil a). admit.
-
-  	    specialize (IHvpqs (fun typD => (existT (typD ts nil) a va)::nil)).
-  	    specialize (IHvpqs (a::nil)).
-  	    Print sigT.
-  	    Check HList.Hnil (typD ts nil).
-  	    specialize (IHvpqs HList.Hnil).
-  	    Print env.
-  	    unfold exprD in IHvpqs. simpl in *.
-  	    SearchAbout env.
-  	    Check @HList.Hnil.
-  	    Check @join_env.
-  	    specialize (IHvpqs (@join_env _ _ (a::nil) (HList.Hnil))).
-  	    rewrite IHvpqs.
-  	    SearchAbout Abs exprD.
-  	    Print Ltac red_exprD.
-  	    SearchAbout Abs.
-  	    Print exprD_rw.
-  	    autorewrite with exprD_rw.
-  	    rewrite exprD_Abs_is_arr.
-  	    simpl in x2.
-  	    red_exprD.
-  	    SearchAbout exprD Inj.
-  	    Print expr.
-  	    rewrite exprD_Inj.
-  	    red_exprD.
-  	    generalize dependent gs.
-  	  Check exprD_Abs.
-  	  SearchAbout exprD Abs.
-  	  rewrite exprD_Abs.
-  	    simpl.
-  	  SearchAbout typ_cast_typ.
-  	  rewrite typeof_expr_exprD_same_type.
-  	  SearchAbout exprD typeof_expr.
-SearchAbout exprD App.
-  	 apply Hp.
-  Qed.
-
-  Definition TR (us vs : env (typD ts)) (r : R Rbase) (t : T) v: Prop :=
-  exists v',
-    exprD us vs (T_to_expr t (typeForR typeForRbase r)) (typeForR typeForRbase r) = Some v' /\
-    @RD r v v'.
-
-Lemma typeof_expr_exprDR (e : expr ilfunc) (t : typ) v
-     (Hexpr : exprD us vs e t = Some v) :
-     WellTyped_expr (typeof_env us) (typeof_env vs) e t.
-Proof.
-	apply typeof_expr_exprD. exists v. apply Hexpr.
-Qed.
-
-  Lemma Happ : forall t1 t2 r1 r2 v1 f,
-  exprD us vs f (typeForR typeForRbase (Rfunctorial t1 t2)) = Some v1 ->
-       @TR us vs (Rfunctorial t1 t2) r1 ->
-       @TR us vs t1 r2 ->
-       @TR us vs t2 (app r1 r2).
-  Proof.
-  	intros t1 t2 r1 r2 f v1 Hexpr [v2 [H1expr H1RD]] [v3 [H2expr H2RD]].
-	simpl in H1RD.
-	specialize (H1RD _ _ H2RD).
-	exists (v2 v3). split; [|apply H1RD].
-	apply T_to_expr_app. assumption. assumption.
-	rewrite <- H2expr.
-	apply H2expr.
-	simpl.
-  	apply typeof_expr_exprDR in H1expr.
-  	apply typeof_expr_exprDR in H2expr.
-  	pose proof (T_to_expr_app_wt H1expr H2expr) as Hexpr3.
-  	apply typeof_expr_exprD in Hexpr3. destruct Hexpr3 as [v Hexpr3].
-  	exists v. split. apply Hexpr3.
-	simpl in H1RD.
-	specialize (H1RD _ _ H2RD).
-	Lemma exprD_RD_app e1 e2 e12 t12 t1 t2 v12 v1 v2 v12' v1'
-	    (H12 : exprD us vs (T_to_expr e12 t12) (typeForR typeForRbase (Rfunctorial t1 t2)) = Some v12)
-		(HRD12 : @RD (Rfunctorial t1 t2) v12 v12')
-		(HRD1 : @RD t1 v1 v1')
-	    (H1 : exprD us vs (T_to_expr e1 (typeForR typeForRbase t1)) (typeForR typeForRbase t1) = Some v1)
-		(H2 : exprD us vs (T_to_expr (app e1 e2) (typeForR typeForRbase t2)) (typeForR typeForRbase t2) = Some v2) :
-		@RD t2 (v12 v1) v2.
-
-  	generalize dependent v'1.
-
-  	exists vpq.
-  	split. apply H3.
-  	eexists. split. apply H3.
-
-    Lemma RD_functorial t1 t2 r1 r2 f g
-    	(H1 : @RD (Rfunctorial t1 t2) r2) (Hr2 : r2 f g) (H2 : @RD t1 r1) :
-    	@RD t2 (fun a b => forall x y, r1 x y -> a = (f x) /\ b = (g y)).
-    Proof.
-    	eapply H1. eassumption.
-    	specialize (H1 (fun a b => forall x y, r1 x y -> a = (f x) /\ b = (g y)) f g Hr2).
-   	    apply H1. simpl. in
-  	eexists.
-
-
-
-
-  Fixpoint pull_exists_left (p : expr ilfunc) : (list typ * expr ilfunc) :=
-  	match p with
-  	  | App (App (Inj (ilf_and t)) p) q =>
-  	  	let (vsp, ep) := pull_exists_left p in
-  	  	let (vsq, eq) := pull_exists_left q in
-  	  		(vsp ++ vsq, App (App (Inj (ilf_and t)) (lift 0 (length vsq) ep)) eq)
-  	  | App (App (Inj (ilf_or t)) p) q =>
-  	  	let (vsp, ep) := pull_exists_left p in
-  	  	let (vsq, eq) := pull_exists_left q in
-  	  		(vsp ++ vsq, App (App (Inj (ilf_or t)) (lift 0 (length vsq) ep)) eq)
-  	  | App (Inj (ilf_exists a _)) (Abs _ f) =>
-  	  		let (vs, e) := pull_exists_left f in (a::vs, e)
-  	  | _ => (nil, p)
-    end.
-
-    Fixpoint apply_exists_aux (t : typ) (vs : list typ)  (e : expr ilfunc) :=
-    match vs with
-    	| nil => e
-		| v :: vs => App (Inj (ilf_exists v t)) (Abs v (apply_exists_aux t vs e))
-	end.
-
-	Definition apply_exists (t : typ) (x : list typ * expr ilfunc) :=
-		apply_exists_aux t (fst x) (snd x).
-
-  	Lemma sound_aux us vs e t v x (H2 : exprD us vs e t = Some v) (ILO : ILogicOps (typD ts nil t))
-  	(_ : gs t = Some ILO)
-  	(_ : exprD us vs e t = Some x) :
-  	v |-- x.
-  	Proof.
-  		unfold apply_exists in H1; simpl in *.
-  		specialize (H t); rewrite H0 in H.
-  		rewrite H1 in H2; inv_all; subst.
-  		Require Import Setoid.
-  		admit.
-  	Qed.
-	Hint Extern 0 (Injective (typ_cast_typ ?A ?B ?C ?D ?E = Some ?F)) =>
-	  eapply (Injective_typ_cast_typ_hetero_Some A B C D E F) : typeclass_instances.
-
-  Lemma exists_pull_left_sound us (t : typ) (ILO : ILogicOps (typD ts nil t))
-    (_ : gs t = Some ILO) (p : expr ilfunc) : forall vs v x
-    (_ : exprD us vs p t = Some v)
-  	(_ : exprD us vs (apply_exists t (pull_exists_left p)) t = Some x),
-  	@lentails (typD ts nil t) ILO v x.
-  Proof.
-  	apply expr_strong_ind with (e := p); clear p; intros.
-  	destruct e; simpl in *; eauto using sound_aux.
-  	destruct e1; simpl in *; eauto using sound_aux.
-  	destruct i; simpl in *; eauto using sound_aux.
-  	destruct e2; simpl in *; eauto using sound_aux.
-  	progress (repeat autorewrite with exprD_rw in H2); simpl in H2.
-  	forward. inv_all; revert H9; subst; intros.
-  	red_exprD. unfold funcAs in H6; simpl in H6. forward.
-  	simpl in *. inv_all; subst.
-  		  repeat (match goal with
-	  		   | H : exists x, _ |- _ => destruct H; intuition; subst
-	  		  end).
-	  		  uip_all.
-	Check exprD_App.
-	rewrite (@exprD_App ts ilfunc RSym_ilfunc us vs (tyArr t0 t) t2 e2) in H7.
-	rewrite exprD_App with (RSym_func := RSym_ilfunc) in H7.
-	Check exprD_App.
-	Check RSym_ilfunc.
-	Check RSym_func.
-	rewrite exprD_App in H7.
-	+ red. solve_expr_acc_trans.
-	+
-	setoid_rewrite <- pull_exists_left.
-  	red_exprD.
-  	unfold apply_exists. simpl. exists v. intuition. admit.
-  	unfold apply_exists. simpl. exists v. intuition. admit.
-    destruct
-  Qed.
+            Lemma pt_quant_sym {A B C : Type} {ILOps : ILogicOps C} {IL : ILogic C} vars pt (e : A -> B -> C) :
+               (var_entail vars _) (pt_quant pt _ (fun x => pt_quant pt _ (fun y => e x y))) (pt_quant pt _ (fun x => pt_quant pt _ (fun y => e y x))). 
+            Proof.
+              destruct vars; (destruct pt; simpl; [
+                do 2 (apply lforallR; intros); do 2 (eapply lforallL); reflexivity |
+                do 2 (apply lexistsL; intros); do 2 (eapply lexistsR); reflexivity
+              ]).
+            Qed.
+            transitivity ((pt_quant pt (ILogic_Ops_fold_fun (t:=t) ILOps typs0)
+     						(fun v0 : hlist (typD ts nil) (rev xs) =>
+    					     t3 us (hlist_app v0 vs) (t7 us vs)))).
+
+         Lemma pt_quant_elim vars {A B : Type} {ILOps : ILogicOps A} {IL : ILogic A} pt (e1 e2 : B -> A) (H : forall x, (var_entail vars _) (e1 x) (e2 x)) :
+         	(var_entail vars _) (pt_quant pt _ e1) (pt_quant pt _ e2).
+         Proof.
+           destruct vars; (destruct pt; simpl in *; unfold flip in *; [
+           apply lforallR; intro x; apply lforallL with x; apply H |
+           apply lexistsL; intro x; apply lexistsR with x; apply H]).
+         Qed.
+
+         apply pt_quant_elim. intros.
+         transitivity (t3 us (hlist_app x3 vs) (t2 us vs)).
+         replace l with (l ++ nil) in H22 by (apply app_nil_r).
+         pose proof (exprD'_add_quants_app_Some H1 H22).
+         destruct H28 as [? [? ?]].
+         pose proof (@exprD'_add_quants_rev_Some t0 _ p H1 tus l tvs _ _ H28).
+         destruct H30 as [? [? ?]]. simpl in *.
+         assert (Some t4 = Some x4) by intuition congruence.
+         inv_all; subst.
+         specialize (H29 us vs).
+         etransitivity; [eapply H25|].
+         eapply H27.
+         rewrite H29.
+         apply pt_quant_elim; intros.
+         reflexivity.
+         eapply H27.
+         destruct v; simpl in *; apply H24.
+         clear -H19.
+         specialize (H19 us vs); destruct vars; [destruct H19 as [_ H19] | destruct H19 as [H19 _]]; simpl in *; specialize (H19 (t7 us vs)).
+ 
 
 End PullExistsLeft.
 
